# Chapter 7.3: Properties and Identities of Inverse Trigonometric Functions

## Overview

Inverse trigonometric functions satisfy numerous important properties and identities that are essential for simplification, evaluation, and problem-solving. These identities connect inverse trig functions to each other and to algebraic expressions.

---

## ğŸ“ Fundamental Composition Properties

### Type 1: f(fâ»Â¹(x)) = x

$$\sin(\sin^{-1}x) = x, \quad x \in [-1, 1]$$

$$\cos(\cos^{-1}x) = x, \quad x \in [-1, 1]$$

$$\tan(\tan^{-1}x) = x, \quad x \in \mathbb{R}$$

```
    â”Œâ”€â”€â”€â”€â”€â”€â”€â”€â”€â”€â”€â”€â”€â”€â”€â”€â”€â”€â”€â”€â”€â”€â”€â”€â”€â”€â”€â”€â”€â”€â”€â”€â”€â”€â”€â”€â”€â”€â”€â”€â”€â”€â”€â”€â”€â”€â”€â”€â”€â”€â”€â”€â”€â”€â”€â”€â”€â”€â”€â”€â”€â”
    â”‚                                                             â”‚
    â”‚   These work for ALL x in the DOMAIN of the inverse        â”‚
    â”‚                                                             â”‚
    â”‚   Think: "Taking inverse then applying function"           â”‚
    â”‚          always gets you back to where you started         â”‚
    â”‚                                                             â”‚
    â””â”€â”€â”€â”€â”€â”€â”€â”€â”€â”€â”€â”€â”€â”€â”€â”€â”€â”€â”€â”€â”€â”€â”€â”€â”€â”€â”€â”€â”€â”€â”€â”€â”€â”€â”€â”€â”€â”€â”€â”€â”€â”€â”€â”€â”€â”€â”€â”€â”€â”€â”€â”€â”€â”€â”€â”€â”€â”€â”€â”€â”€â”˜
```

### Type 2: fâ»Â¹(f(x)) = x (with restrictions!)

$$\sin^{-1}(\sin\theta) = \theta, \quad \theta \in [-\frac{\pi}{2}, \frac{\pi}{2}]$$

$$\cos^{-1}(\cos\theta) = \theta, \quad \theta \in [0, \pi]$$

$$\tan^{-1}(\tan\theta) = \theta, \quad \theta \in (-\frac{\pi}{2}, \frac{\pi}{2})$$

```
    âš ï¸ CRITICAL RESTRICTION âš ï¸
    
    These only work when Î¸ is in the RANGE of the inverse function!
    
    Example: sinâ»Â¹(sin(2Ï€)) â‰  2Ï€  (since 2Ï€ âˆ‰ [-Ï€/2, Ï€/2])
             sinâ»Â¹(sin(2Ï€)) = sinâ»Â¹(0) = 0
```

---

## ğŸ“ The Complementary Relationships

### Sum Equals Ï€/2 or Ï€

$$\boxed{\sin^{-1}x + \cos^{-1}x = \frac{\pi}{2}, \quad |x| \leq 1}$$

$$\boxed{\tan^{-1}x + \cot^{-1}x = \frac{\pi}{2}, \quad x \in \mathbb{R}}$$

$$\boxed{\sec^{-1}x + \csc^{-1}x = \frac{\pi}{2}, \quad |x| \geq 1}$$

### Proof of sinâ»Â¹x + cosâ»Â¹x = Ï€/2

```
    Let sinâ»Â¹x = Î¸, where Î¸ âˆˆ [-Ï€/2, Ï€/2]
    
    Then sin Î¸ = x
    
    cos(Ï€/2 - Î¸) = sin Î¸ = x
    
    Since Î¸ âˆˆ [-Ï€/2, Ï€/2], we have (Ï€/2 - Î¸) âˆˆ [0, Ï€]
    
    So Ï€/2 - Î¸ = cosâ»Â¹x
    
    Therefore: Î¸ + cosâ»Â¹x = Ï€/2
               sinâ»Â¹x + cosâ»Â¹x = Ï€/2  âˆ
```

---

## ğŸ“ Negative Argument Properties

### Odd Functions (negation goes through)

$$\boxed{\sin^{-1}(-x) = -\sin^{-1}x}$$

$$\boxed{\tan^{-1}(-x) = -\tan^{-1}x}$$

$$\boxed{\csc^{-1}(-x) = -\csc^{-1}x}$$

### Special Functions (negation shifts by Ï€)

$$\boxed{\cos^{-1}(-x) = \pi - \cos^{-1}x}$$

$$\boxed{\sec^{-1}(-x) = \pi - \sec^{-1}x}$$

$$\boxed{\cot^{-1}(-x) = \pi - \cot^{-1}x}$$

### Visual Understanding

```
    For odd functions:
    
         y                        sinâ»Â¹(-x) = -sinâ»Â¹x
         â”‚                        
     Ï€/2 â”¤           *            Point (a, b) reflects to
         â”‚         *              point (-a, -b)
       0 â”¼â”€â”€â”€â”€â”€â”€â”€*â”€â”€â”€â”€â”€â”€â”€â”€x
         â”‚     *                  
    -Ï€/2 â”¤   *
         â”‚
    
    For cosâ»Â¹:
    
         y                        cosâ»Â¹(-x) = Ï€ - cosâ»Â¹x
         â”‚
       Ï€ â”¤ *                      If cosâ»Â¹(a) = b
         â”‚   *                    Then cosâ»Â¹(-a) = Ï€ - b
    Ï€/2  â”¤â”€â”€â”€â”€â”€*â”€â”€â”€â”€
         â”‚       *                Point (a, b) relates to
       0 â”¤         *              point (-a, Ï€-b)
         â””â”€â”€â”€â”€â”€â”€â”€â”€â”€â”€â”€â”€â”€ x
          -1       1
```

---

## ğŸ“ Reciprocal Argument Identities

### For |x| â‰¥ 1

$$\boxed{\sin^{-1}\left(\frac{1}{x}\right) = \csc^{-1}x}$$

$$\boxed{\cos^{-1}\left(\frac{1}{x}\right) = \sec^{-1}x}$$

### For All x â‰  0

$$\tan^{-1}\left(\frac{1}{x}\right) = \begin{cases} \cot^{-1}x = \frac{\pi}{2} - \tan^{-1}x & \text{if } x > 0 \\ \cot^{-1}x - \pi = -\frac{\pi}{2} - \tan^{-1}x & \text{if } x < 0 \end{cases}$$

### Simplified Form for x > 0

$$\boxed{\tan^{-1}x + \tan^{-1}\left(\frac{1}{x}\right) = \frac{\pi}{2}, \quad x > 0}$$

$$\boxed{\tan^{-1}x + \tan^{-1}\left(\frac{1}{x}\right) = -\frac{\pi}{2}, \quad x < 0}$$

---

## ğŸ“ Addition Formulas for tanâ»Â¹

### Sum Formula

$$\boxed{\tan^{-1}x + \tan^{-1}y = \tan^{-1}\left(\frac{x+y}{1-xy}\right) + \begin{cases} 0 & \text{if } xy < 1 \\ \pi & \text{if } xy > 1, x > 0 \\ -\pi & \text{if } xy > 1, x < 0 \end{cases}}$$

### Simplified (Most Common Case: xy < 1)

$$\boxed{\tan^{-1}x + \tan^{-1}y = \tan^{-1}\left(\frac{x+y}{1-xy}\right), \quad xy < 1}$$

### Difference Formula

$$\boxed{\tan^{-1}x - \tan^{-1}y = \tan^{-1}\left(\frac{x-y}{1+xy}\right), \quad xy > -1}$$

### Proof of Sum Formula (xy < 1)

```
    Let tanâ»Â¹x = Î± and tanâ»Â¹y = Î²
    
    Then tan Î± = x and tan Î² = y
    
    tan(Î± + Î²) = (tan Î± + tan Î²)/(1 - tan Î± tan Î²)
                = (x + y)/(1 - xy)
    
    If xy < 1, then (Î± + Î²) âˆˆ (-Ï€/2, Ï€/2), so:
    
    Î± + Î² = tanâ»Â¹((x + y)/(1 - xy))
    
    tanâ»Â¹x + tanâ»Â¹y = tanâ»Â¹((x + y)/(1 - xy))  âˆ
```

---

## ğŸ“ Double and Half Value Formulas

### Double Value

$$\boxed{2\tan^{-1}x = \tan^{-1}\left(\frac{2x}{1-x^2}\right), \quad |x| < 1}$$

$$\boxed{2\tan^{-1}x = \sin^{-1}\left(\frac{2x}{1+x^2}\right), \quad |x| \leq 1}$$

$$\boxed{2\tan^{-1}x = \cos^{-1}\left(\frac{1-x^2}{1+x^2}\right), \quad x \geq 0}$$

### Derivation of 2tanâ»Â¹x = sinâ»Â¹(2x/(1+xÂ²))

```
    Let tanâ»Â¹x = Î¸, so tan Î¸ = x
    
    Then: sin 2Î¸ = 2 tan Î¸/(1 + tanÂ²Î¸) = 2x/(1 + xÂ²)
    
    So: 2Î¸ = sinâ»Â¹(2x/(1 + xÂ²))
    
    Therefore: 2tanâ»Â¹x = sinâ»Â¹(2x/(1 + xÂ²))  âˆ
```

---

## ğŸ“ Special Values and Sums

### Important Special Sums

$$\tan^{-1}1 + \tan^{-1}2 + \tan^{-1}3 = \pi$$

$$\tan^{-1}\frac{1}{2} + \tan^{-1}\frac{1}{3} = \frac{\pi}{4}$$

$$\tan^{-1}1 + \tan^{-1}\frac{1}{2} + \tan^{-1}\frac{1}{3} = \frac{\pi}{2}$$

### Proof: tanâ»Â¹(1/2) + tanâ»Â¹(1/3) = Ï€/4

```
    tanâ»Â¹(1/2) + tanâ»Â¹(1/3) = tanâ»Â¹((1/2 + 1/3)/(1 - 1/6))
    
                            = tanâ»Â¹((5/6)/(5/6))
                            
                            = tanâ»Â¹(1)
                            
                            = Ï€/4  âˆ
```

---

## ğŸ“ Inverse Trigonometric Functions with Algebraic Expressions

### Converting Between Forms

For x âˆˆ [-1, 1]:

$$\sin^{-1}x = \cos^{-1}\sqrt{1-x^2}, \quad x \geq 0$$

$$\sin^{-1}x = -\cos^{-1}\sqrt{1-x^2}, \quad x < 0$$

$$\sin^{-1}x = \tan^{-1}\frac{x}{\sqrt{1-x^2}}, \quad |x| < 1$$

### Geometric Interpretation

```
    If sinâ»Â¹x = Î¸, then sin Î¸ = x = x/1
    
    Drawing a right triangle:
    
              /|
             / |
          1 /  | x
           /   |
          /Î¸   |
         /_____|
         âˆš(1-xÂ²)
    
    From this triangle:
    
    cos Î¸ = âˆš(1-xÂ²)/1 = âˆš(1-xÂ²)
    tan Î¸ = x/âˆš(1-xÂ²)
    
    Therefore:
    sinâ»Â¹x = Î¸ = cosâ»Â¹(âˆš(1-xÂ²)) = tanâ»Â¹(x/âˆš(1-xÂ²))
```

---

## ğŸ“ Worked Examples

### Example 1: Simplify sinâ»Â¹(sin 5Ï€/6)

**Solution:**
5Ï€/6 is NOT in [-Ï€/2, Ï€/2], so we can't directly say the answer is 5Ï€/6.

```
    sin(5Ï€/6) = sin(Ï€ - Ï€/6) = sin(Ï€/6) = 1/2
    
    sinâ»Â¹(sin 5Ï€/6) = sinâ»Â¹(1/2) = Ï€/6
```

**Answer: Ï€/6**

---

### Example 2: Prove that tanâ»Â¹(1/2) + tanâ»Â¹(1/5) + tanâ»Â¹(1/8) = Ï€/4

**Solution:**
Use the addition formula twice:

```
    First, combine tanâ»Â¹(1/2) + tanâ»Â¹(1/5):
    
    = tanâ»Â¹((1/2 + 1/5)/(1 - 1/10))
    = tanâ»Â¹((7/10)/(9/10))
    = tanâ»Â¹(7/9)
    
    Now add tanâ»Â¹(1/8):
    
    tanâ»Â¹(7/9) + tanâ»Â¹(1/8) = tanâ»Â¹((7/9 + 1/8)/(1 - 7/72))
    
    Numerator: 7/9 + 1/8 = 56/72 + 9/72 = 65/72
    
    Denominator: 1 - 7/72 = 65/72
    
    = tanâ»Â¹((65/72)/(65/72))
    = tanâ»Â¹(1)
    = Ï€/4  âˆ
```

---

### Example 3: Express tanâ»Â¹(cos x/(1 + sin x)) in simplest form

**Solution:**

```
    Use the half-angle substitution approach:
    
    cos x = cosÂ²(x/2) - sinÂ²(x/2)
    1 + sin x = 1 + 2 sin(x/2) cos(x/2)
              = sinÂ²(x/2) + cosÂ²(x/2) + 2 sin(x/2) cos(x/2)
              = (cos(x/2) + sin(x/2))Â²
    
    cos x/(1 + sin x) = (cos(x/2) - sin(x/2))(cos(x/2) + sin(x/2))
                        â”€â”€â”€â”€â”€â”€â”€â”€â”€â”€â”€â”€â”€â”€â”€â”€â”€â”€â”€â”€â”€â”€â”€â”€â”€â”€â”€â”€â”€â”€â”€â”€â”€â”€â”€â”€â”€â”€â”€â”€â”€â”€â”€â”€â”€
                                (cos(x/2) + sin(x/2))Â²
    
                      = (cos(x/2) - sin(x/2))/(cos(x/2) + sin(x/2))
    
    Divide numerator and denominator by cos(x/2):
    
                      = (1 - tan(x/2))/(1 + tan(x/2))
    
                      = tan(Ï€/4 - x/2)
```

**Answer: tanâ»Â¹(cos x/(1 + sin x)) = Ï€/4 - x/2**

---

### Example 4: If sinâ»Â¹x + sinâ»Â¹y = Ï€/2, prove xÂ² + yÂ² = 1

**Solution:**

```
    sinâ»Â¹x + sinâ»Â¹y = Ï€/2
    
    sinâ»Â¹y = Ï€/2 - sinâ»Â¹x = cosâ»Â¹x    [using the complementary identity]
    
    y = sin(cosâ»Â¹x)
    
    If cosâ»Â¹x = Î¸, then cos Î¸ = x
    sin Î¸ = âˆš(1 - cosÂ²Î¸) = âˆš(1 - xÂ²)
    
    So y = âˆš(1 - xÂ²)
    
    Therefore: yÂ² = 1 - xÂ²
    
    xÂ² + yÂ² = 1  âˆ
```

---

## ğŸ“‹ Summary Table

### Key Identities

| Identity | Condition | Notes |
|----------|-----------|-------|
| sinâ»Â¹x + cosâ»Â¹x = Ï€/2 | \|x\| â‰¤ 1 | Complementary pair |
| tanâ»Â¹x + cotâ»Â¹x = Ï€/2 | x âˆˆ â„ | Complementary pair |
| sinâ»Â¹(-x) = -sinâ»Â¹x | \|x\| â‰¤ 1 | Odd function |
| cosâ»Â¹(-x) = Ï€ - cosâ»Â¹x | \|x\| â‰¤ 1 | Shift property |
| tanâ»Â¹(-x) = -tanâ»Â¹x | x âˆˆ â„ | Odd function |
| tanâ»Â¹x + tanâ»Â¹(1/x) = Ï€/2 | x > 0 | Reciprocal sum |
| tanâ»Â¹x + tanâ»Â¹y = tanâ»Â¹((x+y)/(1-xy)) | xy < 1 | Addition formula |
| 2tanâ»Â¹x = tanâ»Â¹(2x/(1-xÂ²)) | \|x\| < 1 | Double angle |

### Composition Rules

| Composition | Result | Condition |
|-------------|--------|-----------|
| sin(sinâ»Â¹x) | x | \|x\| â‰¤ 1 |
| sinâ»Â¹(sin Î¸) | Î¸ | Î¸ âˆˆ [-Ï€/2, Ï€/2] |
| cos(cosâ»Â¹x) | x | \|x\| â‰¤ 1 |
| cosâ»Â¹(cos Î¸) | Î¸ | Î¸ âˆˆ [0, Ï€] |
| tan(tanâ»Â¹x) | x | x âˆˆ â„ |
| tanâ»Â¹(tan Î¸) | Î¸ | Î¸ âˆˆ (-Ï€/2, Ï€/2) |

---

## â“ Quick Revision Questions

1. **Evaluate: cosâ»Â¹(cos 4Ï€/3)**

2. **Simplify: tanâ»Â¹(1) + tanâ»Â¹(2) + tanâ»Â¹(3)**

3. **If tanâ»Â¹x + tanâ»Â¹y = Ï€/4, express y in terms of x.**

4. **Prove: sinâ»Â¹(3/5) + sinâ»Â¹(4/5) = Ï€/2**

5. **Evaluate: tanâ»Â¹(1/2) + tanâ»Â¹(1/3)**

6. **Express 2tanâ»Â¹(1/3) as a single inverse function.**

<details>
<summary>Click to see answers</summary>

1. **cosâ»Â¹(cos 4Ï€/3)**
   
   4Ï€/3 is NOT in [0, Ï€], so we need to adjust.
   
   cos(4Ï€/3) = cos(Ï€ + Ï€/3) = -cos(Ï€/3) = -1/2
   
   cosâ»Â¹(-1/2) = **2Ï€/3**

2. **tanâ»Â¹(1) + tanâ»Â¹(2) + tanâ»Â¹(3)**
   
   First: tanâ»Â¹(1) + tanâ»Â¹(2) = Ï€/4 + tanâ»Â¹(2)
   
   = tanâ»Â¹((1+2)/(1-2)) + Ï€  [since xy = 2 > 1 and x > 0]
   = tanâ»Â¹(-3) + Ï€
   = Ï€ - tanâ»Â¹(3)
   
   Adding tanâ»Â¹(3):
   Ï€ - tanâ»Â¹(3) + tanâ»Â¹(3) = **Ï€**

3. **tanâ»Â¹x + tanâ»Â¹y = Ï€/4**
   
   tanâ»Â¹y = Ï€/4 - tanâ»Â¹x = tanâ»Â¹((1-x)/(1+x))  [assuming 1Â·x < 1]
   
   **y = (1-x)/(1+x)**

4. **sinâ»Â¹(3/5) + sinâ»Â¹(4/5) = Ï€/2**
   
   Note that (3/5)Â² + (4/5)Â² = 9/25 + 16/25 = 25/25 = 1
   
   So 4/5 = âˆš(1 - (3/5)Â²), which means:
   sinâ»Â¹(4/5) = cosâ»Â¹(3/5)
   
   Therefore: sinâ»Â¹(3/5) + sinâ»Â¹(4/5) = sinâ»Â¹(3/5) + cosâ»Â¹(3/5) = **Ï€/2** âˆ

5. **tanâ»Â¹(1/2) + tanâ»Â¹(1/3)**
   
   = tanâ»Â¹((1/2 + 1/3)/(1 - 1/6))
   = tanâ»Â¹((5/6)/(5/6))
   = tanâ»Â¹(1)
   = **Ï€/4**

6. **2tanâ»Â¹(1/3)**
   
   Using 2tanâ»Â¹x = tanâ»Â¹(2x/(1-xÂ²)):
   
   = tanâ»Â¹(2(1/3)/(1 - 1/9))
   = tanâ»Â¹((2/3)/(8/9))
   = tanâ»Â¹((2/3)(9/8))
   = **tanâ»Â¹(3/4)**

</details>

---

## Navigation

| Previous | Up | Next |
|----------|-------|------|
| [â† 7.2 Graphs of Inverse Functions](02-graphs.md) | [Unit 7 Index](README.md) | [7.4 Applications â†’](04-applications.md) |

---

[â† Back to Main Index](../README.md)
