# Chapter 8.2: Laws of Exponents

[â† Previous: Exponents Basics](01-exponents-basics.md) | [Back to Contents](../README.md) | [Next: Square and Cube Roots â†’](03-square-cube-roots.md)

---

## ğŸ¯ Learning Objectives

By the end of this chapter, you will be able to:
- Apply the product rule for exponents
- Apply the quotient rule for exponents
- Work with power of a power
- Simplify complex expressions using exponent laws

---

## 1. Overview of Exponent Laws

### The Seven Laws
```
â”Œâ”€â”€â”€â”€â”€â”€â”€â”€â”€â”€â”€â”€â”€â”€â”€â”€â”€â”€â”€â”€â”€â”€â”€â”€â”€â”€â”€â”€â”€â”€â”€â”€â”€â”€â”€â”€â”€â”€â”€â”€â”€â”€â”€â”€â”€â”€â”€â”€â”€â”€â”€â”€â”€â”€â”€â”€â”€â”
â”‚                  LAWS OF EXPONENTS                      â”‚
â”œâ”€â”€â”€â”€â”€â”€â”€â”€â”€â”€â”€â”€â”€â”€â”€â”€â”€â”€â”€â”€â”€â”€â”€â”€â”€â”€â”€â”€â”€â”€â”€â”€â”€â”€â”€â”€â”€â”€â”€â”€â”€â”€â”€â”€â”€â”€â”€â”€â”€â”€â”€â”€â”€â”€â”€â”€â”€â”¤
â”‚                                                         â”‚
â”‚  1. Product Rule:     aáµ Ã— aâ¿ = aáµâºâ¿                   â”‚
â”‚                                                         â”‚
â”‚  2. Quotient Rule:    aáµ Ã· aâ¿ = aáµâ»â¿                   â”‚
â”‚                                                         â”‚
â”‚  3. Power Rule:       (aáµ)â¿ = aáµâ¿                      â”‚
â”‚                                                         â”‚
â”‚  4. Power of Product: (ab)â¿ = aâ¿bâ¿                     â”‚
â”‚                                                         â”‚
â”‚  5. Power of Quotient: (a/b)â¿ = aâ¿/bâ¿                  â”‚
â”‚                                                         â”‚
â”‚  6. Zero Exponent:    aâ° = 1 (a â‰  0)                   â”‚
â”‚                                                         â”‚
â”‚  7. Negative Exponent: aâ»â¿ = 1/aâ¿                      â”‚
â”‚                                                         â”‚
â””â”€â”€â”€â”€â”€â”€â”€â”€â”€â”€â”€â”€â”€â”€â”€â”€â”€â”€â”€â”€â”€â”€â”€â”€â”€â”€â”€â”€â”€â”€â”€â”€â”€â”€â”€â”€â”€â”€â”€â”€â”€â”€â”€â”€â”€â”€â”€â”€â”€â”€â”€â”€â”€â”€â”€â”€â”€â”˜
```

---

## 2. Law 1: Product Rule

### The Rule
```
When multiplying powers with the SAME BASE:
ADD the exponents.

aáµ Ã— aâ¿ = aáµâºâ¿
```

### Why It Works
```
2Â³ Ã— 2â´ = (2 Ã— 2 Ã— 2) Ã— (2 Ã— 2 Ã— 2 Ã— 2)
        = 2 Ã— 2 Ã— 2 Ã— 2 Ã— 2 Ã— 2 Ã— 2
        = 2â· = 2Â³âºâ´
```

### Examples
```
3Â² Ã— 3âµ = 3Â²âºâµ = 3â· = 2187

xâ´ Ã— xÂ³ = xâ´âºÂ³ = xâ·

5Â³ Ã— 5 = 5Â³ Ã— 5Â¹ = 5â´ = 625

2â»Â² Ã— 2âµ = 2â»Â²âºâµ = 2Â³ = 8

aáµ Ã— aâ¿ Ã— aáµ– = aáµâºâ¿âºáµ–
```

### Common Mistakes
```
âŒ 2Â³ Ã— 3Â² = 6âµ  WRONG! (Different bases)
âœ“ 2Â³ Ã— 3Â² = 8 Ã— 9 = 72

âŒ 5Â² Ã— 5Â³ = 5â¶  WRONG! (Multiplied exponents)
âœ“ 5Â² Ã— 5Â³ = 5âµ = 3125

Remember: Add exponents, don't multiply!
```

---

## 3. Law 2: Quotient Rule

### The Rule
```
When dividing powers with the SAME BASE:
SUBTRACT the exponents.

aáµ Ã· aâ¿ = aáµâ»â¿  OR  aáµ/aâ¿ = aáµâ»â¿
```

### Why It Works
```
2âµ Ã· 2Â³ = (2 Ã— 2 Ã— 2 Ã— 2 Ã— 2) Ã· (2 Ã— 2 Ã— 2)
        = 2 Ã— 2
        = 2Â² = 2âµâ»Â³
```

### Examples
```
5â· Ã· 5â´ = 5â·â»â´ = 5Â³ = 125

xâ¸/xÂ³ = xâ¸â»Â³ = xâµ

10â¶/10â¶ = 10â¶â»â¶ = 10â° = 1

3Â² Ã· 3âµ = 3Â²â»âµ = 3â»Â³ = 1/27

aâ´ Ã· aâ»Â² = aâ´â»â½â»Â²â¾ = aâ´âºÂ² = aâ¶
```

### Visual Understanding
```
2âµ Ã· 2Â² = ?

2âµ = 2 Ã— 2 Ã— 2 Ã— 2 Ã— 2
     â”€â”€â”€â”€â”€â”€â”€â”€â”€â”€â”€â”€â”€â”€â”€â”€â”€
2Â² =         2 Ã— 2

Cancel 2 factors: 2 Ã— 2 Ã— 2 = 2Â³ = 2âµâ»Â²
```

---

## 4. Law 3: Power of a Power

### The Rule
```
When raising a power to another power:
MULTIPLY the exponents.

(aáµ)â¿ = aáµË£â¿
```

### Why It Works
```
(2Â³)Â² = 2Â³ Ã— 2Â³
      = (2 Ã— 2 Ã— 2) Ã— (2 Ã— 2 Ã— 2)
      = 2â¶ = 2Â³Ë£Â²
```

### Examples
```
(3Â²)â´ = 3Â²Ë£â´ = 3â¸ = 6561

(xâµ)Â³ = xâµË£Â³ = xÂ¹âµ

(2â»Â³)Â² = 2â»Â³Ë£Â² = 2â»â¶ = 1/64

(aâ´)â»Â² = aâ´Ë£â½â»Â²â¾ = aâ»â¸ = 1/aâ¸

((xÂ²)Â³)â´ = xÂ²Ë£Â³Ë£â´ = xÂ²â´
```

### Distinction from Product Rule
```
Product Rule:   aáµ Ã— aâ¿ = aáµâºâ¿  (ADD)
Power Rule:     (aáµ)â¿ = aáµË£â¿    (MULTIPLY)

2Â³ Ã— 2â´ = 2â·   (3 + 4 = 7)
(2Â³)â´ = 2Â¹Â²    (3 Ã— 4 = 12)
```

---

## 5. Law 4: Power of a Product

### The Rule
```
When raising a product to a power:
Raise each factor to that power.

(ab)â¿ = aâ¿bâ¿
```

### Why It Works
```
(2 Ã— 3)Â² = (2 Ã— 3) Ã— (2 Ã— 3)
         = 2 Ã— 2 Ã— 3 Ã— 3
         = 2Â² Ã— 3Â² = 4 Ã— 9 = 36

Check: (2 Ã— 3)Â² = 6Â² = 36 âœ“
```

### Examples
```
(2x)Â³ = 2Â³ Ã— xÂ³ = 8xÂ³

(3ab)Â² = 3Â² Ã— aÂ² Ã— bÂ² = 9aÂ²bÂ²

(5xyÂ²)Â³ = 5Â³ Ã— xÂ³ Ã— (yÂ²)Â³ = 125xÂ³yâ¶

(-2a)â´ = (-2)â´ Ã— aâ´ = 16aâ´

(2aÂ³b)Â² = 4aâ¶bÂ²
```

### Reverse Application
```
Factor out common powers:

8xÂ³ = (2x)Â³
27aÂ³bÂ³ = (3ab)Â³
64xâ¶ = (4xÂ²)Â³ = (2x)â¶
```

---

## 6. Law 5: Power of a Quotient

### The Rule
```
When raising a quotient to a power:
Raise numerator and denominator to that power.

(a/b)â¿ = aâ¿/bâ¿
```

### Examples
```
(2/3)â´ = 2â´/3â´ = 16/81

(x/y)Â³ = xÂ³/yÂ³

(3/x)Â² = 9/xÂ²

(2a/3b)Â³ = (2a)Â³/(3b)Â³ = 8aÂ³/27bÂ³

(aÂ²/bÂ³)â´ = aâ¸/bÂ¹Â²
```

### Negative Exponents
```
(a/b)â»â¿ = (b/a)â¿ = bâ¿/aâ¿

(2/3)â»Â² = (3/2)Â² = 9/4

(x/y)â»Â³ = yÂ³/xÂ³
```

---

## 7. Combining Multiple Laws

### Example 1
```
Simplify: (xÂ³yÂ²)â´

Step 1: Apply power of product
= xÂ³Ë£â´ Ã— yÂ²Ë£â´
= xÂ¹Â² Ã— yâ¸
= xÂ¹Â²yâ¸
```

### Example 2
```
Simplify: (2aÂ²bÂ³)Â³ Ã· (4abÂ²)Â²

Step 1: Expand each term
(2aÂ²bÂ³)Â³ = 8aâ¶bâ¹
(4abÂ²)Â² = 16aÂ²bâ´

Step 2: Divide
= 8aâ¶bâ¹ / 16aÂ²bâ´
= (8/16) Ã— aâ¶â»Â² Ã— bâ¹â»â´
= (1/2) Ã— aâ´ Ã— bâµ
= aâ´bâµ/2
```

### Example 3
```
Simplify: (xâ´yâ»Â²)Â³ Ã— (xâ»Â²yÂ³)Â²

Step 1: Expand each term
(xâ´yâ»Â²)Â³ = xÂ¹Â²yâ»â¶
(xâ»Â²yÂ³)Â² = xâ»â´yâ¶

Step 2: Multiply
= xÂ¹Â² Ã— xâ»â´ Ã— yâ»â¶ Ã— yâ¶
= xÂ¹Â²â»â´ Ã— yâ»â¶âºâ¶
= xâ¸ Ã— yâ°
= xâ¸ Ã— 1
= xâ¸
```

### Example 4
```
Simplify: (3xÂ²/yÂ³)Â² Ã— (y/x)â´

Step 1: Expand
(3xÂ²/yÂ³)Â² = 9xâ´/yâ¶
(y/x)â´ = yâ´/xâ´

Step 2: Multiply
= (9xâ´/yâ¶) Ã— (yâ´/xâ´)
= 9xâ´yâ´ / yâ¶xâ´
= 9 Ã— xâ´â»â´ Ã— yâ´â»â¶
= 9 Ã— xâ° Ã— yâ»Â²
= 9/yÂ²
```

---

## 8. Working with Numerical Expressions

### Example 1
```
Calculate: 2âµ Ã— 2Â³ Ã· 2â¶

= 2âµâºÂ³â»â¶
= 2Â²
= 4
```

### Example 2
```
Calculate: (3Â²)Â³ Ã· 3â´

= 3â¶ Ã· 3â´
= 3â¶â»â´
= 3Â²
= 9
```

### Example 3
```
Simplify: 12â¶/6Â³

Method 1: Factor the base
12 = 2Â² Ã— 3, 6 = 2 Ã— 3

12â¶/6Â³ = (2Â² Ã— 3)â¶/(2 Ã— 3)Â³
       = 2Â¹Â² Ã— 3â¶ / 2Â³ Ã— 3Â³
       = 2Â¹Â²â»Â³ Ã— 3â¶â»Â³
       = 2â¹ Ã— 3Â³
       = 512 Ã— 27
       = 13,824

Method 2: Direct calculation
12â¶/6Â³ = 12â¶/6Â³ = (12/6)Â² Ã— 12â´ = 2Â² Ã— 12â´
       = 4 Ã— 20,736 = ... (more complex)
```

### Example 4
```
Simplify: 8Â³ Ã— 4Â²/2â·

Express all in powers of 2:
8 = 2Â³, 4 = 2Â²

= (2Â³)Â³ Ã— (2Â²)Â²/2â·
= 2â¹ Ã— 2â´/2â·
= 2â¹âºâ´â»â·
= 2â¶
= 64
```

---

## 9. Laws Summary with Memory Aids

### Visual Summary
```
â•”â•â•â•â•â•â•â•â•â•â•â•â•â•â•â•â•â•â•â•â•â•â•â•â•â•â•â•â•â•â•â•â•â•â•â•â•â•â•â•â•â•â•â•â•â•â•â•â•â•â•â•â•â•â•â•â•—
â•‘   SAME BASE:                                          â•‘
â•‘   Multiply â†’ ADD exponents      aáµ Ã— aâ¿ = aáµâºâ¿       â•‘
â•‘   Divide â†’ SUBTRACT exponents   aáµ Ã· aâ¿ = aáµâ»â¿       â•‘
â•‘                                                       â•‘
â•‘   POWER OF POWER:                                     â•‘
â•‘   â†’ MULTIPLY exponents          (aáµ)â¿ = aáµâ¿          â•‘
â•‘                                                       â•‘
â•‘   DISTRIBUTE POWER:                                   â•‘
â•‘   Over products                 (ab)â¿ = aâ¿bâ¿         â•‘
â•‘   Over quotients               (a/b)â¿ = aâ¿/bâ¿        â•‘
â•‘                                                       â•‘
â•‘   SPECIAL CASES:                                      â•‘
â•‘   Zero exponent                 aâ° = 1               â•‘
â•‘   Negative exponent             aâ»â¿ = 1/aâ¿           â•‘
â•šâ•â•â•â•â•â•â•â•â•â•â•â•â•â•â•â•â•â•â•â•â•â•â•â•â•â•â•â•â•â•â•â•â•â•â•â•â•â•â•â•â•â•â•â•â•â•â•â•â•â•â•â•â•â•â•â•
```

### Memory Tricks
```
"Same Base, Add for Multiply"
"Same Base, Subtract for Divide"
"Stacked Powers Multiply"

For (ab)â¿: "Power distributes like multiplication"

For aâ»â¿: "Negative goes down" (to denominator)
```

---

## 10. Solved Examples

### Example 1: Product Rule
```
Simplify: xâµ Ã— xâ»Â² Ã— xÂ³

= xâµâºâ½â»Â²â¾âºÂ³
= xâ¶
```

### Example 2: Quotient Rule
```
Simplify: aâ·bÂ³/(aÂ²bâµ)

= aâ·â»Â² Ã— bÂ³â»âµ
= aâµ Ã— bâ»Â²
= aâµ/bÂ²
```

### Example 3: Power Rule
```
Simplify: [(xÂ²)Â³]Â²

= [xâ¶]Â²
= xÂ¹Â²
```

### Example 4: Combined
```
Simplify: (2xÂ³y)Â² Ã— (3xyÂ²)Â³

= (4xâ¶yÂ²) Ã— (27xÂ³yâ¶)
= 4 Ã— 27 Ã— xâ¶âºÂ³ Ã— yÂ²âºâ¶
= 108xâ¹yâ¸
```

### Example 5: With Negative Exponents
```
Simplify: (xâ»Â²yÂ³)â»Â² Ã· (xâ´yâ»Â¹)

= xâ´yâ»â¶ Ã· xâ´yâ»Â¹
= xâ´â»â´ Ã— yâ»â¶â»â½â»Â¹â¾
= xâ° Ã— yâ»â¶âºÂ¹
= yâ»âµ
= 1/yâµ
```

### Example 6: Numerical
```
Calculate: 27Â² Ã— 3â´/81Â²

Express all as powers of 3:
27 = 3Â³, 81 = 3â´

= (3Â³)Â² Ã— 3â´/(3â´)Â²
= 3â¶ Ã— 3â´/3â¸
= 3â¶âºâ´â»â¸
= 3Â²
= 9
```

---

## 11. Mental Math Tips ğŸ§ 

### Quick Exponent Addition
```
For aáµ Ã— aâ¿, just add m + n:

xÂ³ Ã— xâµ â†’ 3 + 5 = 8 â†’ xâ¸
2â´ Ã— 2â¶ â†’ 4 + 6 = 10 â†’ 2Â¹â°
```

### Power of Power Shortcut
```
For (aáµ)â¿, multiply m Ã— n:

(xÂ²)âµ â†’ 2 Ã— 5 = 10 â†’ xÂ¹â°
(2Â³)â´ â†’ 3 Ã— 4 = 12 â†’ 2Â¹Â²
```

### Negative Exponent Flip
```
Move base to opposite side, change sign:

xâ»Â³ in numerator â†’ xÂ³ in denominator
yâ»Â² in denominator â†’ yÂ² in numerator

xâ»Â³/yâ»Â² = yÂ²/xÂ³
```

### Express in Powers of 2 or 3
```
4 = 2Â², 8 = 2Â³, 16 = 2â´, 32 = 2âµ
9 = 3Â², 27 = 3Â³, 81 = 3â´

This makes complex calculations simpler!
```

---

## ğŸ“Š Summary Table

### Laws Quick Reference

| Law | Rule | Example |
|-----|------|---------|
| Product | aáµ Ã— aâ¿ = aáµâºâ¿ | xÂ² Ã— xÂ³ = xâµ |
| Quotient | aáµ Ã· aâ¿ = aáµâ»â¿ | xâµ Ã· xÂ² = xÂ³ |
| Power | (aáµ)â¿ = aáµâ¿ | (xÂ²)Â³ = xâ¶ |
| Product Power | (ab)â¿ = aâ¿bâ¿ | (2x)Â³ = 8xÂ³ |
| Quotient Power | (a/b)â¿ = aâ¿/bâ¿ | (x/2)Â² = xÂ²/4 |
| Zero | aâ° = 1 | 5â° = 1 |
| Negative | aâ»â¿ = 1/aâ¿ | 2â»Â³ = 1/8 |

### Common Errors to Avoid

| Wrong âŒ | Right âœ“ |
|----------|---------|
| 2Â³ Ã— 2â´ = 2Â¹Â² | 2Â³ Ã— 2â´ = 2â· |
| (2Â³)â´ = 2â· | (2Â³)â´ = 2Â¹Â² |
| 2Â³ Ã— 3Â² = 6âµ | 2Â³ Ã— 3Â² = 8 Ã— 9 = 72 |
| (2 + 3)Â² = 2Â² + 3Â² | (2 + 3)Â² = 5Â² = 25 |

---

## â“ Quick Revision Questions

1. **Simplify**: xâ´ Ã— xâµ

2. **Simplify**: yâ¸ Ã· yÂ³

3. **Simplify**: (aÂ³)â´

4. **Simplify**: (2xyÂ²)Â³

5. **Simplify**: 4âµ Ã— 4â»Â² Ã· 4Â²

6. **Simplify**: (xÂ²yâ»Â³)â´ Ã· (xy)Â²

<details>
<summary>Click to see answers</summary>

1. xâ´ Ã— xâµ = xâ´âºâµ = **xâ¹**

2. yâ¸ Ã· yÂ³ = yâ¸â»Â³ = **yâµ**

3. (aÂ³)â´ = aÂ³Ë£â´ = **aÂ¹Â²**

4. (2xyÂ²)Â³ = 2Â³xÂ³yâ¶ = **8xÂ³yâ¶**

5. 4âµ Ã— 4â»Â² Ã· 4Â² = 4âµâ»Â²â»Â² = 4Â¹ = **4**

6. (xÂ²yâ»Â³)â´ Ã· (xy)Â²
   = xâ¸yâ»Â¹Â² Ã· xÂ²yÂ²
   = xâ¸â»Â²yâ»Â¹Â²â»Â²
   = xâ¶yâ»Â¹â´
   = **xâ¶/yÂ¹â´**

</details>

---

## ğŸ”— Navigation

[â† Previous: Exponents Basics](01-exponents-basics.md) | [Back to Contents](../README.md) | [Next: Square and Cube Roots â†’](03-square-cube-roots.md)
