# Chapter 6.3: Completing the Square

[â† Previous: Square Root Method](02-square-root-method.md) | [Back to Contents](../README.md) | [Next: The Quadratic Formula â†’](04-quadratic-formula.md)

---

## ğŸ“š Chapter Overview

**Completing the square** is a powerful algebraic technique that transforms any quadratic expression into a perfect square trinomial. This method always works and leads directly to the derivation of the quadratic formula.

---

## ğŸ¯ Learning Objectives

By the end of this chapter, you will be able to:
- Understand what makes a perfect square trinomial
- Find the constant to complete the square
- Solve quadratic equations by completing the square
- Handle equations where a â‰  1
- Use completing the square to find the vertex form
- Derive the quadratic formula

---

## 1. Perfect Square Trinomials

### The Pattern

```
â”Œâ”€â”€â”€â”€â”€â”€â”€â”€â”€â”€â”€â”€â”€â”€â”€â”€â”€â”€â”€â”€â”€â”€â”€â”€â”€â”€â”€â”€â”€â”€â”€â”€â”€â”€â”€â”€â”€â”€â”€â”€â”€â”€â”€â”€â”€â”€â”€â”€â”€â”€â”€â”€â”€â”€â”€â”€â”€â”€â”€â”€â”€â”€â”€â”€â”€â”€â”€â”€â”€â”
â”‚              PERFECT SQUARE TRINOMIAL                               â”‚
â”œâ”€â”€â”€â”€â”€â”€â”€â”€â”€â”€â”€â”€â”€â”€â”€â”€â”€â”€â”€â”€â”€â”€â”€â”€â”€â”€â”€â”€â”€â”€â”€â”€â”€â”€â”€â”€â”€â”€â”€â”€â”€â”€â”€â”€â”€â”€â”€â”€â”€â”€â”€â”€â”€â”€â”€â”€â”€â”€â”€â”€â”€â”€â”€â”€â”€â”€â”€â”€â”€â”¤
â”‚                                                                     â”‚
â”‚   A perfect square trinomial has the form:                        â”‚
â”‚                                                                     â”‚
â”‚   (x + k)Â² = xÂ² + 2kx + kÂ²                                        â”‚
â”‚                                                                     â”‚
â”‚   (x - k)Â² = xÂ² - 2kx + kÂ²                                        â”‚
â”‚                                                                     â”‚
â”‚   Key relationship:                                                â”‚
â”‚   â”Œâ”€â”€â”€â”€â”€â”€â”€â”€â”€â”€â”€â”€â”€â”€â”€â”€â”€â”€â”€â”€â”€â”€â”€â”€â”€â”€â”€â”€â”€â”€â”€â”€â”€â”€â”€â”€â”€â”€â”€â”€â”€â”€â”€â”€â”€â”€â”€â”€â”€â”€â”€â”€â”€â”€â”€â”€â”€â”€â”€â”€â”€â” â”‚
â”‚   â”‚                                                             â”‚ â”‚
â”‚   â”‚   constant term = (half of the linear coefficient)Â²        â”‚ â”‚
â”‚   â”‚                                                             â”‚ â”‚
â”‚   â”‚              kÂ² = (2k/2)Â² = (b/2)Â²                         â”‚ â”‚
â”‚   â”‚                                                             â”‚ â”‚
â”‚   â””â”€â”€â”€â”€â”€â”€â”€â”€â”€â”€â”€â”€â”€â”€â”€â”€â”€â”€â”€â”€â”€â”€â”€â”€â”€â”€â”€â”€â”€â”€â”€â”€â”€â”€â”€â”€â”€â”€â”€â”€â”€â”€â”€â”€â”€â”€â”€â”€â”€â”€â”€â”€â”€â”€â”€â”€â”€â”€â”€â”€â”€â”˜ â”‚
â”‚                                                                     â”‚
â”‚   Examples:                                                        â”‚
â”‚   â€¢ xÂ² + 6x + 9 = (x + 3)Â²    because 9 = (6/2)Â² = 3Â²            â”‚
â”‚   â€¢ xÂ² - 10x + 25 = (x - 5)Â²  because 25 = (10/2)Â² = 5Â²          â”‚
â”‚   â€¢ xÂ² + 4x + 4 = (x + 2)Â²    because 4 = (4/2)Â² = 2Â²            â”‚
â”‚                                                                     â”‚
â””â”€â”€â”€â”€â”€â”€â”€â”€â”€â”€â”€â”€â”€â”€â”€â”€â”€â”€â”€â”€â”€â”€â”€â”€â”€â”€â”€â”€â”€â”€â”€â”€â”€â”€â”€â”€â”€â”€â”€â”€â”€â”€â”€â”€â”€â”€â”€â”€â”€â”€â”€â”€â”€â”€â”€â”€â”€â”€â”€â”€â”€â”€â”€â”€â”€â”€â”€â”€â”€â”˜
```

### Visual Understanding

```
â”Œâ”€â”€â”€â”€â”€â”€â”€â”€â”€â”€â”€â”€â”€â”€â”€â”€â”€â”€â”€â”€â”€â”€â”€â”€â”€â”€â”€â”€â”€â”€â”€â”€â”€â”€â”€â”€â”€â”€â”€â”€â”€â”€â”€â”€â”€â”€â”€â”€â”€â”€â”€â”€â”€â”€â”€â”€â”€â”€â”€â”€â”€â”€â”€â”€â”€â”€â”€â”€â”€â”
â”‚              GEOMETRIC INTERPRETATION                               â”‚
â”œâ”€â”€â”€â”€â”€â”€â”€â”€â”€â”€â”€â”€â”€â”€â”€â”€â”€â”€â”€â”€â”€â”€â”€â”€â”€â”€â”€â”€â”€â”€â”€â”€â”€â”€â”€â”€â”€â”€â”€â”€â”€â”€â”€â”€â”€â”€â”€â”€â”€â”€â”€â”€â”€â”€â”€â”€â”€â”€â”€â”€â”€â”€â”€â”€â”€â”€â”€â”€â”€â”¤
â”‚                                                                     â”‚
â”‚   To complete xÂ² + 6x to a perfect square:                        â”‚
â”‚                                                                     â”‚
â”‚   â”Œâ”€â”€â”€â”€â”€â”€â”€â”€â”€â”€â”€â”¬â”€â”€â”€â”€â”€â”€â”€â”                                            â”‚
â”‚   â”‚           â”‚       â”‚                                            â”‚
â”‚   â”‚    xÂ²     â”‚  3x   â”‚  â† x Ã— 3                                  â”‚
â”‚   â”‚           â”‚       â”‚                                            â”‚
â”‚   â”œâ”€â”€â”€â”€â”€â”€â”€â”€â”€â”€â”€â”¼â”€â”€â”€â”€â”€â”€â”€â”¤                                            â”‚
â”‚   â”‚    3x     â”‚  ?    â”‚  â† 3 Ã— 3 = 9 (needed to complete square) â”‚
â”‚   â”‚           â”‚       â”‚                                            â”‚
â”‚   â””â”€â”€â”€â”€â”€â”€â”€â”€â”€â”€â”€â”´â”€â”€â”€â”€â”€â”€â”€â”˜                                            â”‚
â”‚        x         3                                                  â”‚
â”‚                                                                     â”‚
â”‚   The missing corner has area 3Â² = 9                              â”‚
â”‚                                                                     â”‚
â”‚   So: xÂ² + 6x + 9 = (x + 3)Â²                                      â”‚
â”‚                                                                     â”‚
â””â”€â”€â”€â”€â”€â”€â”€â”€â”€â”€â”€â”€â”€â”€â”€â”€â”€â”€â”€â”€â”€â”€â”€â”€â”€â”€â”€â”€â”€â”€â”€â”€â”€â”€â”€â”€â”€â”€â”€â”€â”€â”€â”€â”€â”€â”€â”€â”€â”€â”€â”€â”€â”€â”€â”€â”€â”€â”€â”€â”€â”€â”€â”€â”€â”€â”€â”€â”€â”€â”˜
```

---

## 2. Finding the Constant to Complete the Square

### The Formula

```
â”Œâ”€â”€â”€â”€â”€â”€â”€â”€â”€â”€â”€â”€â”€â”€â”€â”€â”€â”€â”€â”€â”€â”€â”€â”€â”€â”€â”€â”€â”€â”€â”€â”€â”€â”€â”€â”€â”€â”€â”€â”€â”€â”€â”€â”€â”€â”€â”€â”€â”€â”€â”€â”€â”€â”€â”€â”€â”€â”€â”€â”€â”€â”€â”€â”€â”€â”€â”€â”€â”€â”
â”‚              COMPLETING THE SQUARE FORMULA                          â”‚
â”œâ”€â”€â”€â”€â”€â”€â”€â”€â”€â”€â”€â”€â”€â”€â”€â”€â”€â”€â”€â”€â”€â”€â”€â”€â”€â”€â”€â”€â”€â”€â”€â”€â”€â”€â”€â”€â”€â”€â”€â”€â”€â”€â”€â”€â”€â”€â”€â”€â”€â”€â”€â”€â”€â”€â”€â”€â”€â”€â”€â”€â”€â”€â”€â”€â”€â”€â”€â”€â”€â”¤
â”‚                                                                     â”‚
â”‚   To complete xÂ² + bx to a perfect square:                        â”‚
â”‚                                                                     â”‚
â”‚   Add (b/2)Â² to make:  xÂ² + bx + (b/2)Â² = (x + b/2)Â²             â”‚
â”‚                                                                     â”‚
â”‚   Step 1: Take half of b                                          â”‚
â”‚   Step 2: Square it                                               â”‚
â”‚   Step 3: Add to the expression                                   â”‚
â”‚                                                                     â”‚
â”‚   â”€â”€â”€â”€â”€â”€â”€â”€â”€â”€â”€â”€â”€â”€â”€â”€â”€â”€â”€â”€â”€â”€â”€â”€â”€â”€â”€â”€â”€â”€â”€â”€â”€â”€â”€â”€â”€â”€â”€â”€â”€â”€â”€â”€â”€â”€â”€â”€â”€â”€â”€â”€â”€â”€â”€â”€â”€â”€â”€â”€â”€â”€  â”‚
â”‚                                                                     â”‚
â”‚   Examples:                                                        â”‚
â”‚                                                                     â”‚
â”‚   xÂ² + 8x â†’ need (8/2)Â² = 16 â†’ xÂ² + 8x + 16 = (x + 4)Â²          â”‚
â”‚                                                                     â”‚
â”‚   xÂ² - 12x â†’ need (-12/2)Â² = 36 â†’ xÂ² - 12x + 36 = (x - 6)Â²      â”‚
â”‚                                                                     â”‚
â”‚   xÂ² + 5x â†’ need (5/2)Â² = 25/4 â†’ xÂ² + 5x + 25/4 = (x + 5/2)Â²    â”‚
â”‚                                                                     â”‚
â”‚   xÂ² - 3x â†’ need (-3/2)Â² = 9/4 â†’ xÂ² - 3x + 9/4 = (x - 3/2)Â²     â”‚
â”‚                                                                     â”‚
â””â”€â”€â”€â”€â”€â”€â”€â”€â”€â”€â”€â”€â”€â”€â”€â”€â”€â”€â”€â”€â”€â”€â”€â”€â”€â”€â”€â”€â”€â”€â”€â”€â”€â”€â”€â”€â”€â”€â”€â”€â”€â”€â”€â”€â”€â”€â”€â”€â”€â”€â”€â”€â”€â”€â”€â”€â”€â”€â”€â”€â”€â”€â”€â”€â”€â”€â”€â”€â”€â”˜
```

---

## 3. Solving Equations by Completing the Square

### Step-by-Step Process

```
â”Œâ”€â”€â”€â”€â”€â”€â”€â”€â”€â”€â”€â”€â”€â”€â”€â”€â”€â”€â”€â”€â”€â”€â”€â”€â”€â”€â”€â”€â”€â”€â”€â”€â”€â”€â”€â”€â”€â”€â”€â”€â”€â”€â”€â”€â”€â”€â”€â”€â”€â”€â”€â”€â”€â”€â”€â”€â”€â”€â”€â”€â”€â”€â”€â”€â”€â”€â”€â”€â”€â”
â”‚              SOLVING BY COMPLETING THE SQUARE                       â”‚
â”œâ”€â”€â”€â”€â”€â”€â”€â”€â”€â”€â”€â”€â”€â”€â”€â”€â”€â”€â”€â”€â”€â”€â”€â”€â”€â”€â”€â”€â”€â”€â”€â”€â”€â”€â”€â”€â”€â”€â”€â”€â”€â”€â”€â”€â”€â”€â”€â”€â”€â”€â”€â”€â”€â”€â”€â”€â”€â”€â”€â”€â”€â”€â”€â”€â”€â”€â”€â”€â”€â”¤
â”‚                                                                     â”‚
â”‚   Step 1: Move the constant term to the right side                â”‚
â”‚           xÂ² + bx = -c                                             â”‚
â”‚                                                                     â”‚
â”‚   Step 2: Find (b/2)Â²                                              â”‚
â”‚                                                                     â”‚
â”‚   Step 3: Add (b/2)Â² to BOTH sides                                â”‚
â”‚           xÂ² + bx + (b/2)Â² = -c + (b/2)Â²                          â”‚
â”‚                                                                     â”‚
â”‚   Step 4: Factor the left side as a perfect square                â”‚
â”‚           (x + b/2)Â² = -c + (b/2)Â²                                 â”‚
â”‚                                                                     â”‚
â”‚   Step 5: Take the square root of both sides (Â±)                  â”‚
â”‚           x + b/2 = Â±âˆš(-c + (b/2)Â²)                               â”‚
â”‚                                                                     â”‚
â”‚   Step 6: Solve for x                                              â”‚
â”‚           x = -b/2 Â± âˆš(-c + (b/2)Â²)                               â”‚
â”‚                                                                     â”‚
â””â”€â”€â”€â”€â”€â”€â”€â”€â”€â”€â”€â”€â”€â”€â”€â”€â”€â”€â”€â”€â”€â”€â”€â”€â”€â”€â”€â”€â”€â”€â”€â”€â”€â”€â”€â”€â”€â”€â”€â”€â”€â”€â”€â”€â”€â”€â”€â”€â”€â”€â”€â”€â”€â”€â”€â”€â”€â”€â”€â”€â”€â”€â”€â”€â”€â”€â”€â”€â”€â”˜
```

### Detailed Example

```
Solve: xÂ² + 6x - 7 = 0

Step 1: Move constant to right side
        xÂ² + 6x = 7

Step 2: Find (b/2)Â² = (6/2)Â² = 9

Step 3: Add 9 to both sides
        xÂ² + 6x + 9 = 7 + 9
        xÂ² + 6x + 9 = 16

Step 4: Factor left side
        (x + 3)Â² = 16

Step 5: Take square root
        x + 3 = Â±4

Step 6: Solve for x
        x = -3 + 4 = 1
        x = -3 - 4 = -7

Check:
x = 1: (1)Â² + 6(1) - 7 = 1 + 6 - 7 = 0 âœ“
x = -7: (-7)Â² + 6(-7) - 7 = 49 - 42 - 7 = 0 âœ“

Solutions: x = 1 or x = -7
```

---

## 4. When the Leading Coefficient a â‰  1

### Handling Coefficients

```
â”Œâ”€â”€â”€â”€â”€â”€â”€â”€â”€â”€â”€â”€â”€â”€â”€â”€â”€â”€â”€â”€â”€â”€â”€â”€â”€â”€â”€â”€â”€â”€â”€â”€â”€â”€â”€â”€â”€â”€â”€â”€â”€â”€â”€â”€â”€â”€â”€â”€â”€â”€â”€â”€â”€â”€â”€â”€â”€â”€â”€â”€â”€â”€â”€â”€â”€â”€â”€â”€â”€â”
â”‚              WHEN a â‰  1                                             â”‚
â”œâ”€â”€â”€â”€â”€â”€â”€â”€â”€â”€â”€â”€â”€â”€â”€â”€â”€â”€â”€â”€â”€â”€â”€â”€â”€â”€â”€â”€â”€â”€â”€â”€â”€â”€â”€â”€â”€â”€â”€â”€â”€â”€â”€â”€â”€â”€â”€â”€â”€â”€â”€â”€â”€â”€â”€â”€â”€â”€â”€â”€â”€â”€â”€â”€â”€â”€â”€â”€â”€â”¤
â”‚                                                                     â”‚
â”‚   For axÂ² + bx + c = 0 where a â‰  1:                               â”‚
â”‚                                                                     â”‚
â”‚   Step 0: Divide ENTIRE equation by a first!                      â”‚
â”‚           xÂ² + (b/a)x + (c/a) = 0                                  â”‚
â”‚                                                                     â”‚
â”‚   Then proceed with completing the square on xÂ² + (b/a)x          â”‚
â”‚                                                                     â”‚
â”‚   â”€â”€â”€â”€â”€â”€â”€â”€â”€â”€â”€â”€â”€â”€â”€â”€â”€â”€â”€â”€â”€â”€â”€â”€â”€â”€â”€â”€â”€â”€â”€â”€â”€â”€â”€â”€â”€â”€â”€â”€â”€â”€â”€â”€â”€â”€â”€â”€â”€â”€â”€â”€â”€â”€â”€â”€â”€â”€â”€â”€â”€â”€  â”‚
â”‚                                                                     â”‚
â”‚   Example: 2xÂ² + 12x - 14 = 0                                     â”‚
â”‚                                                                     â”‚
â”‚   Step 0: Divide by 2                                             â”‚
â”‚           xÂ² + 6x - 7 = 0                                          â”‚
â”‚                                                                     â”‚
â”‚   Now proceed as before (same as previous example)                â”‚
â”‚                                                                     â”‚
â””â”€â”€â”€â”€â”€â”€â”€â”€â”€â”€â”€â”€â”€â”€â”€â”€â”€â”€â”€â”€â”€â”€â”€â”€â”€â”€â”€â”€â”€â”€â”€â”€â”€â”€â”€â”€â”€â”€â”€â”€â”€â”€â”€â”€â”€â”€â”€â”€â”€â”€â”€â”€â”€â”€â”€â”€â”€â”€â”€â”€â”€â”€â”€â”€â”€â”€â”€â”€â”€â”˜
```

### Another Example with a â‰  1

```
Solve: 3xÂ² - 6x - 9 = 0

Step 0: Divide by 3
        xÂ² - 2x - 3 = 0

Step 1: xÂ² - 2x = 3

Step 2: (b/2)Â² = (-2/2)Â² = 1

Step 3: xÂ² - 2x + 1 = 3 + 1 = 4

Step 4: (x - 1)Â² = 4

Step 5: x - 1 = Â±2

Step 6: x = 1 + 2 = 3  or  x = 1 - 2 = -1

Solutions: x = 3 or x = -1
```

---

## 5. Equations with Irrational Solutions

### When the Right Side Isn't a Perfect Square

```
Solve: xÂ² + 4x - 1 = 0

Step 1: xÂ² + 4x = 1

Step 2: (4/2)Â² = 4

Step 3: xÂ² + 4x + 4 = 1 + 4 = 5

Step 4: (x + 2)Â² = 5

Step 5: x + 2 = Â±âˆš5

Step 6: x = -2 Â± âˆš5

Solutions: x = -2 + âˆš5 â‰ˆ 0.236
          x = -2 - âˆš5 â‰ˆ -4.236
```

---

## 6. Equations with No Real Solutions

### When the Right Side is Negative

```
Solve: xÂ² + 2x + 5 = 0

Step 1: xÂ² + 2x = -5

Step 2: (2/2)Â² = 1

Step 3: xÂ² + 2x + 1 = -5 + 1 = -4

Step 4: (x + 1)Â² = -4

Step 5: x + 1 = Â±âˆš(-4)

Cannot take square root of negative number in real numbers!

NO REAL SOLUTIONS
(Complex solutions: x = -1 Â± 2i)
```

---

## 7. Vertex Form of a Quadratic

### Converting to Vertex Form

```
â”Œâ”€â”€â”€â”€â”€â”€â”€â”€â”€â”€â”€â”€â”€â”€â”€â”€â”€â”€â”€â”€â”€â”€â”€â”€â”€â”€â”€â”€â”€â”€â”€â”€â”€â”€â”€â”€â”€â”€â”€â”€â”€â”€â”€â”€â”€â”€â”€â”€â”€â”€â”€â”€â”€â”€â”€â”€â”€â”€â”€â”€â”€â”€â”€â”€â”€â”€â”€â”€â”€â”
â”‚              VERTEX FORM                                            â”‚
â”œâ”€â”€â”€â”€â”€â”€â”€â”€â”€â”€â”€â”€â”€â”€â”€â”€â”€â”€â”€â”€â”€â”€â”€â”€â”€â”€â”€â”€â”€â”€â”€â”€â”€â”€â”€â”€â”€â”€â”€â”€â”€â”€â”€â”€â”€â”€â”€â”€â”€â”€â”€â”€â”€â”€â”€â”€â”€â”€â”€â”€â”€â”€â”€â”€â”€â”€â”€â”€â”€â”¤
â”‚                                                                     â”‚
â”‚   Vertex form: y = a(x - h)Â² + k                                  â”‚
â”‚                                                                     â”‚
â”‚   Where (h, k) is the vertex of the parabola                      â”‚
â”‚                                                                     â”‚
â”‚   Completing the square converts standard form to vertex form:    â”‚
â”‚                                                                     â”‚
â”‚   y = xÂ² + 6x + 2                                                  â”‚
â”‚                                                                     â”‚
â”‚   y = (xÂ² + 6x + 9) - 9 + 2    â† Add and subtract 9              â”‚
â”‚   y = (x + 3)Â² - 7                                                 â”‚
â”‚                                                                     â”‚
â”‚   Vertex: (-3, -7)                                                 â”‚
â”‚                                                                     â”‚
â”‚   â”Œâ”€â”€â”€â”€â”€â”€â”€â”€â”€â”€â”€â”€â”€â”€â”€â”€â”€â”€â”€â”€â”€â”€â”€â”€â”€â”€â”€â”€â”€â”€â”€â”€â”€â”€â”€â”€â”€â”€â”€â”€â”€â”€â”€â”                   â”‚
â”‚   â”‚         â”‚                                 â”‚                   â”‚
â”‚   â”‚         â”‚      â•±â•²                        â”‚                   â”‚
â”‚   â”‚         â”‚     â•±  â•²                       â”‚                   â”‚
â”‚   â”‚    â”€â”€â”€â”€â”€â”¼â”€â”€â”€â”€â—â”€â”€â”€â”€â•²â”€â”€â”€â”€â”€                 â”‚                   â”‚
â”‚   â”‚         â”‚   (-3,-7)  â•²                   â”‚                   â”‚
â”‚   â”‚         â”‚             â•²                  â”‚                   â”‚
â”‚   â””â”€â”€â”€â”€â”€â”€â”€â”€â”€â”€â”€â”€â”€â”€â”€â”€â”€â”€â”€â”€â”€â”€â”€â”€â”€â”€â”€â”€â”€â”€â”€â”€â”€â”€â”€â”€â”€â”€â”€â”€â”€â”€â”€â”˜                   â”‚
â”‚                                                                     â”‚
â””â”€â”€â”€â”€â”€â”€â”€â”€â”€â”€â”€â”€â”€â”€â”€â”€â”€â”€â”€â”€â”€â”€â”€â”€â”€â”€â”€â”€â”€â”€â”€â”€â”€â”€â”€â”€â”€â”€â”€â”€â”€â”€â”€â”€â”€â”€â”€â”€â”€â”€â”€â”€â”€â”€â”€â”€â”€â”€â”€â”€â”€â”€â”€â”€â”€â”€â”€â”€â”€â”˜
```

---

## 8. Deriving the Quadratic Formula

### The Derivation

```
Start with: axÂ² + bx + c = 0

Divide by a:
xÂ² + (b/a)x + c/a = 0

Move constant:
xÂ² + (b/a)x = -c/a

Complete the square (add (b/2a)Â² to both sides):
xÂ² + (b/a)x + (b/2a)Â² = -c/a + (b/2a)Â²

Factor left side:
(x + b/2a)Â² = -c/a + bÂ²/4aÂ²

Common denominator on right:
(x + b/2a)Â² = -4ac/4aÂ² + bÂ²/4aÂ²
(x + b/2a)Â² = (bÂ² - 4ac)/4aÂ²

Take square root:
x + b/2a = Â±âˆš(bÂ² - 4ac)/2a

Solve for x:
x = -b/2a Â± âˆš(bÂ² - 4ac)/2a

        â”Œâ”€â”€â”€â”€â”€â”€â”€â”€â”€â”€â”€â”€â”€â”€â”€â”€â”€â”€â”€â”€â”€â”€â”€â”€â”€â”€â”€â”€â”€â”€â”€â”€â”€â”€â”€â”€â”
        â”‚                                    â”‚
        â”‚      -b Â± âˆš(bÂ² - 4ac)             â”‚
        â”‚  x = â”€â”€â”€â”€â”€â”€â”€â”€â”€â”€â”€â”€â”€â”€â”€â”€â”€            â”‚
        â”‚            2a                      â”‚
        â”‚                                    â”‚
        â”‚   THE QUADRATIC FORMULA           â”‚
        â”‚                                    â”‚
        â””â”€â”€â”€â”€â”€â”€â”€â”€â”€â”€â”€â”€â”€â”€â”€â”€â”€â”€â”€â”€â”€â”€â”€â”€â”€â”€â”€â”€â”€â”€â”€â”€â”€â”€â”€â”€â”˜
```

---

## âœï¸ Solved Examples

### Example 1: Easy - Perfect Square Result

**Problem:** Solve xÂ² + 8x + 7 = 0

**Solution:**
```
Step 1: xÂ² + 8x = -7

Step 2: (8/2)Â² = 16

Step 3: xÂ² + 8x + 16 = -7 + 16 = 9

Step 4: (x + 4)Â² = 9

Step 5: x + 4 = Â±3

Step 6: x = -4 + 3 = -1
        x = -4 - 3 = -7

Answer: x = -1 or x = -7
```

### Example 2: Easy - Negative Linear Coefficient

**Problem:** Solve xÂ² - 4x - 5 = 0

**Solution:**
```
Step 1: xÂ² - 4x = 5

Step 2: (-4/2)Â² = 4

Step 3: xÂ² - 4x + 4 = 5 + 4 = 9

Step 4: (x - 2)Â² = 9

Step 5: x - 2 = Â±3

Step 6: x = 2 + 3 = 5
        x = 2 - 3 = -1

Answer: x = 5 or x = -1
```

### Example 3: Medium - Irrational Solutions

**Problem:** Solve xÂ² + 6x + 2 = 0

**Solution:**
```
Step 1: xÂ² + 6x = -2

Step 2: (6/2)Â² = 9

Step 3: xÂ² + 6x + 9 = -2 + 9 = 7

Step 4: (x + 3)Â² = 7

Step 5: x + 3 = Â±âˆš7

Step 6: x = -3 Â± âˆš7

Answer: x = -3 + âˆš7 â‰ˆ -0.354
        x = -3 - âˆš7 â‰ˆ -5.646
```

### Example 4: Medium - Leading Coefficient â‰  1

**Problem:** Solve 2xÂ² + 8x - 10 = 0

**Solution:**
```
Step 0: Divide by 2
        xÂ² + 4x - 5 = 0

Step 1: xÂ² + 4x = 5

Step 2: (4/2)Â² = 4

Step 3: xÂ² + 4x + 4 = 5 + 4 = 9

Step 4: (x + 2)Â² = 9

Step 5: x + 2 = Â±3

Step 6: x = -2 + 3 = 1
        x = -2 - 3 = -5

Answer: x = 1 or x = -5
```

### Example 5: Medium - Fractional Coefficient

**Problem:** Solve xÂ² + 5x + 2 = 0

**Solution:**
```
Step 1: xÂ² + 5x = -2

Step 2: (5/2)Â² = 25/4

Step 3: xÂ² + 5x + 25/4 = -2 + 25/4
                       = -8/4 + 25/4
                       = 17/4

Step 4: (x + 5/2)Â² = 17/4

Step 5: x + 5/2 = Â±âˆš(17/4) = Â±âˆš17/2

Step 6: x = -5/2 Â± âˆš17/2
        x = (-5 Â± âˆš17)/2

Answer: x = (-5 + âˆš17)/2 â‰ˆ -0.438
        x = (-5 - âˆš17)/2 â‰ˆ -4.562
```

### Example 6: Hard - General Case

**Problem:** Solve 3xÂ² - 12x + 7 = 0

**Solution:**
```
Step 0: Divide by 3
        xÂ² - 4x + 7/3 = 0

Step 1: xÂ² - 4x = -7/3

Step 2: (-4/2)Â² = 4

Step 3: xÂ² - 4x + 4 = -7/3 + 4
                    = -7/3 + 12/3
                    = 5/3

Step 4: (x - 2)Â² = 5/3

Step 5: x - 2 = Â±âˆš(5/3) = Â±âˆš15/3

Step 6: x = 2 Â± âˆš15/3

Answer: x = 2 + âˆš15/3 â‰ˆ 3.291
        x = 2 - âˆš15/3 â‰ˆ 0.709
```

---

## â“ Practice Problems

### Easy Level

1. Solve by completing the square: xÂ² + 10x + 16 = 0

2. Solve: xÂ² - 6x + 5 = 0

3. Solve: xÂ² + 2x - 15 = 0

### Medium Level

4. Solve: xÂ² - 8x + 10 = 0

5. Solve: xÂ² + 3x - 2 = 0

6. Solve: 2xÂ² + 12x + 10 = 0

### Hard Level

7. Solve: xÂ² - 5x + 1 = 0

8. Convert to vertex form: y = xÂ² - 4x + 7

9. Solve: 3xÂ² + 6x - 2 = 0

---

## âœ… Answers to Practice Problems

<details>
<summary>Click to reveal answers</summary>

1. xÂ² + 10x = -16, add 25
   (x + 5)Â² = 9
   x + 5 = Â±3
   **x = -2 or x = -8**

2. xÂ² - 6x = -5, add 9
   (x - 3)Â² = 4
   **x = 5 or x = 1**

3. xÂ² + 2x = 15, add 1
   (x + 1)Â² = 16
   **x = 3 or x = -5**

4. xÂ² - 8x = -10, add 16
   (x - 4)Â² = 6
   **x = 4 Â± âˆš6**

5. xÂ² + 3x = 2, add 9/4
   (x + 3/2)Â² = 17/4
   **x = (-3 Â± âˆš17)/2**

6. Divide by 2: xÂ² + 6x + 5 = 0
   xÂ² + 6x = -5, add 9
   (x + 3)Â² = 4
   **x = -1 or x = -5**

7. xÂ² - 5x = -1, add 25/4
   (x - 5/2)Â² = 21/4
   **x = (5 Â± âˆš21)/2**

8. y = (xÂ² - 4x + 4) - 4 + 7
   **y = (x - 2)Â² + 3, vertex: (2, 3)**

9. xÂ² + 2x - 2/3 = 0
   xÂ² + 2x = 2/3, add 1
   (x + 1)Â² = 5/3
   **x = -1 Â± âˆš(5/3) = (-3 Â± âˆš15)/3**

</details>

---

## ğŸ“‹ Summary Table

| Step | Action |
|------|--------|
| 1 | If a â‰  1, divide entire equation by a |
| 2 | Move constant to right side |
| 3 | Find (b/2)Â² |
| 4 | Add (b/2)Â² to both sides |
| 5 | Factor left as (x + b/2)Â² |
| 6 | Take square root (Â±) |
| 7 | Solve for x |

---

## ğŸ”„ Quick Revision Questions

1. **What number completes the square: xÂ² + 12x + ___?**

2. **What is (x + 4)Â² expanded?**

3. **If (x - 3)Â² = 25, what are the solutions?**

4. **What's the first step when a â‰  1?**

5. **What form is y = a(x - h)Â² + k called?**

6. **What does completing the square help derive?**

<details>
<summary>Quick Answers</summary>

1. (12/2)Â² = 36
2. xÂ² + 8x + 16
3. x - 3 = Â±5, so x = 8 or x = -2
4. Divide the entire equation by a
5. Vertex form
6. The quadratic formula

</details>

---

## ğŸ”— Key Takeaways

```
â”Œâ”€â”€â”€â”€â”€â”€â”€â”€â”€â”€â”€â”€â”€â”€â”€â”€â”€â”€â”€â”€â”€â”€â”€â”€â”€â”€â”€â”€â”€â”€â”€â”€â”€â”€â”€â”€â”€â”€â”€â”€â”€â”€â”€â”€â”€â”€â”€â”€â”€â”€â”€â”€â”€â”€â”€â”€â”€â”€â”€â”€â”€â”€â”€â”€â”€â”€â”€â”€â”€â”
â”‚                    CHAPTER SUMMARY                                  â”‚
â”œâ”€â”€â”€â”€â”€â”€â”€â”€â”€â”€â”€â”€â”€â”€â”€â”€â”€â”€â”€â”€â”€â”€â”€â”€â”€â”€â”€â”€â”€â”€â”€â”€â”€â”€â”€â”€â”€â”€â”€â”€â”€â”€â”€â”€â”€â”€â”€â”€â”€â”€â”€â”€â”€â”€â”€â”€â”€â”€â”€â”€â”€â”€â”€â”€â”€â”€â”€â”€â”€â”¤
â”‚                                                                     â”‚
â”‚   â˜… Perfect square: xÂ² + bx + (b/2)Â² = (x + b/2)Â²                â”‚
â”‚                                                                     â”‚
â”‚   â˜… Key formula: Add (b/2)Â² to complete the square                â”‚
â”‚                                                                     â”‚
â”‚   â˜… Process:                                                       â”‚
â”‚     1. Make leading coefficient 1 (divide by a)                   â”‚
â”‚     2. Move constant to right                                     â”‚
â”‚     3. Add (b/2)Â² to both sides                                   â”‚
â”‚     4. Factor as perfect square                                   â”‚
â”‚     5. Take Â± square root                                         â”‚
â”‚     6. Solve for x                                                â”‚
â”‚                                                                     â”‚
â”‚   â˜… Completing the square:                                        â”‚
â”‚     â€¢ Always works (unlike factoring)                             â”‚
â”‚     â€¢ Gives vertex form of parabola                              â”‚
â”‚     â€¢ Derives the quadratic formula                              â”‚
â”‚                                                                     â”‚
â””â”€â”€â”€â”€â”€â”€â”€â”€â”€â”€â”€â”€â”€â”€â”€â”€â”€â”€â”€â”€â”€â”€â”€â”€â”€â”€â”€â”€â”€â”€â”€â”€â”€â”€â”€â”€â”€â”€â”€â”€â”€â”€â”€â”€â”€â”€â”€â”€â”€â”€â”€â”€â”€â”€â”€â”€â”€â”€â”€â”€â”€â”€â”€â”€â”€â”€â”€â”€â”€â”˜
```

---

[â† Previous: Square Root Method](02-square-root-method.md) | [Back to Contents](../README.md) | [Next: The Quadratic Formula â†’](04-quadratic-formula.md)
