# Chapter 2.4: Mathematical Induction

[‚Üê Previous: Proof by Contradiction](03-proof-by-contradiction.md) | [Back to README](../README.md) | [Next: Strong Induction ‚Üí](05-strong-induction.md)

---

## üìã Chapter Overview

**Mathematical induction** is a powerful proof technique for statements involving natural numbers. It works like a chain of dominoes ‚Äî proving the first one falls and that each one knocks down the next guarantees they all fall.

---

## 1. The Principle of Mathematical Induction (PMI)

To prove: $\forall n \geq n_0, \, P(n)$ is true

**Two steps:**

| Step | Name | What to Do |
|------|------|-----------|
| **Step 1** | Base Case | Prove $P(n_0)$ is true |
| **Step 2** | Inductive Step | Prove: if $P(k)$ is true, then $P(k+1)$ is true |

If both steps hold, then $P(n)$ is true for all $n \geq n_0$.

### The Domino Analogy

```
  Base Case        Inductive Step
  (first falls)    (each knocks next)
  
  ‚îå‚îÄ‚îê  ‚îå‚îÄ‚îê  ‚îå‚îÄ‚îê  ‚îå‚îÄ‚îê  ‚îå‚îÄ‚îê  ‚îå‚îÄ‚îê  ‚îå‚îÄ‚îê
  ‚îÇ ‚îÇ  ‚îÇ ‚îÇ  ‚îÇ ‚îÇ  ‚îÇ ‚îÇ  ‚îÇ ‚îÇ  ‚îÇ ‚îÇ  ‚îÇ ‚îÇ  ...
  ‚îÇ ‚îÇ\ ‚îÇ ‚îÇ\ ‚îÇ ‚îÇ\ ‚îÇ ‚îÇ\ ‚îÇ ‚îÇ\ ‚îÇ ‚îÇ\ ‚îÇ ‚îÇ\
  ‚îÇ ‚îÇ \‚îÇ ‚îÇ \‚îÇ ‚îÇ \‚îÇ ‚îÇ \‚îÇ ‚îÇ \‚îÇ ‚îÇ \‚îÇ ‚îÇ \
  ‚îî‚îÄ‚îò  ‚îî‚îÄ‚îò  ‚îî‚îÄ‚îò  ‚îî‚îÄ‚îò  ‚îî‚îÄ‚îò  ‚îî‚îÄ‚îò  ‚îî‚îÄ‚îò
  n‚ÇÄ   n‚ÇÄ+1 n‚ÇÄ+2 n‚ÇÄ+3  ...
  
  P(n‚ÇÄ) ‚Üí P(n‚ÇÄ+1) ‚Üí P(n‚ÇÄ+2) ‚Üí P(n‚ÇÄ+3) ‚Üí ...
```

---

## 2. Why Induction Works

Induction is based on the axiom: if a set $S \subseteq \mathbb{N}$ satisfies:
1. $n_0 \in S$
2. $k \in S \Rightarrow k+1 \in S$

Then $S = \{n_0, n_0+1, n_0+2, \ldots\} = \{n \in \mathbb{N} : n \geq n_0\}$.

---

## 3. Worked Examples

### Example 1: Sum of first $n$ natural numbers

**Theorem:** $\displaystyle\sum_{i=1}^{n} i = \frac{n(n+1)}{2}$ for all $n \geq 1$.

**Base Case ($n = 1$):**
$$\text{LHS} = 1, \quad \text{RHS} = \frac{1 \cdot 2}{2} = 1 \quad \checkmark$$

**Inductive Step:** Assume $P(k)$: $\sum_{i=1}^{k} i = \frac{k(k+1)}{2}$ (Inductive Hypothesis)

Prove $P(k+1)$: $\sum_{i=1}^{k+1} i = \frac{(k+1)(k+2)}{2}$

$$\sum_{i=1}^{k+1} i = \underbrace{\sum_{i=1}^{k} i}_{\text{IH: } \frac{k(k+1)}{2}} + (k+1)$$
$$= \frac{k(k+1)}{2} + (k+1) = \frac{k(k+1) + 2(k+1)}{2} = \frac{(k+1)(k+2)}{2} \quad \checkmark$$

By PMI, the formula holds for all $n \geq 1$. $\blacksquare$

---

### Example 2: Sum of first $n$ squares

**Theorem:** $\displaystyle\sum_{i=1}^{n} i^2 = \frac{n(n+1)(2n+1)}{6}$ for all $n \geq 1$.

**Base Case ($n = 1$):**
$$\text{LHS} = 1, \quad \text{RHS} = \frac{1 \cdot 2 \cdot 3}{6} = 1 \quad \checkmark$$

**Inductive Step:** Assume $\sum_{i=1}^{k} i^2 = \frac{k(k+1)(2k+1)}{6}$.

$$\sum_{i=1}^{k+1} i^2 = \frac{k(k+1)(2k+1)}{6} + (k+1)^2$$
$$= \frac{k(k+1)(2k+1) + 6(k+1)^2}{6}$$
$$= \frac{(k+1)[k(2k+1) + 6(k+1)]}{6}$$
$$= \frac{(k+1)(2k^2 + k + 6k + 6)}{6}$$
$$= \frac{(k+1)(2k^2 + 7k + 6)}{6}$$
$$= \frac{(k+1)(k+2)(2k+3)}{6}$$
$$= \frac{(k+1)((k+1)+1)(2(k+1)+1)}{6} \quad \checkmark$$

$\blacksquare$

---

### Example 3: Divisibility ‚Äî $6 \mid (n^3 - n)$ for all $n \geq 1$

**Base Case ($n = 1$):** $1^3 - 1 = 0 = 6 \cdot 0$ ‚úì

**Inductive Step:** Assume $6 \mid (k^3 - k)$, i.e., $k^3 - k = 6m$ for some integer $m$.

$$(k+1)^3 - (k+1) = k^3 + 3k^2 + 3k + 1 - k - 1$$
$$= (k^3 - k) + 3k^2 + 3k$$
$$= (k^3 - k) + 3k(k + 1)$$

Now, $k(k+1)$ is always even (product of consecutive integers), so $k(k+1) = 2t$.
Thus $3k(k+1) = 6t$.

So $(k+1)^3 - (k+1) = 6m + 6t = 6(m + t)$.

Therefore $6 \mid ((k+1)^3 - (k+1))$. $\blacksquare$

---

### Example 4: Inequality ‚Äî $2^n > n$ for all $n \geq 1$

**Base Case ($n = 1$):** $2^1 = 2 > 1$ ‚úì

**Inductive Step:** Assume $2^k > k$ for some $k \geq 1$.

$$2^{k+1} = 2 \cdot 2^k > 2 \cdot k = k + k \geq k + 1$$

(since $k \geq 1$ implies $k \geq 1$, so $k + k \geq k + 1$)

Therefore $2^{k+1} > k + 1$. $\blacksquare$

---

### Example 5: Geometric series

**Theorem:** $\displaystyle\sum_{i=0}^{n} r^i = \frac{r^{n+1} - 1}{r - 1}$ for $r \neq 1$ and $n \geq 0$.

**Base Case ($n = 0$):**
$$\text{LHS} = r^0 = 1, \quad \text{RHS} = \frac{r - 1}{r - 1} = 1 \quad \checkmark$$

**Inductive Step:** Assume the formula holds for $k$:

$$\sum_{i=0}^{k+1} r^i = \sum_{i=0}^{k} r^i + r^{k+1} = \frac{r^{k+1} - 1}{r - 1} + r^{k+1}$$
$$= \frac{r^{k+1} - 1 + r^{k+1}(r - 1)}{r - 1} = \frac{r^{k+1} - 1 + r^{k+2} - r^{k+1}}{r - 1} = \frac{r^{k+2} - 1}{r - 1} \quad \checkmark$$

$\blacksquare$

---

## 4. Common Mistakes in Induction

| Mistake | Why it's Wrong |
|---------|---------------|
| **Forgetting base case** | Inductive step alone proves nothing |
| **Wrong base case** | Must match the starting value $n_0$ |
| **Not using the inductive hypothesis** | Must explicitly use $P(k)$ to prove $P(k+1)$ |
| **Proving $P(k)$ instead of $P(k+1)$** | Must prove the NEXT case, not the current one |
| **Circular reasoning** | Cannot assume $P(k+1)$ while proving it |

### Classic Trap: "All horses are the same color"

The inductive step fails at the base case $n = 1 \rightarrow n = 2$: when $n = 2$, removing one horse from each end gives two single-horse sets that DON'T overlap. The argument requires overlap, which fails at this critical step.

---

## 5. Proof Template

```
  Theorem: P(n) for all n ‚â• n‚ÇÄ.
  
  Proof (by mathematical induction):
  
  Base Case: [Show P(n‚ÇÄ) is true]
  
  Inductive Hypothesis: Assume P(k) is true for some 
  arbitrary k ‚â• n‚ÇÄ. That is, assume [state P(k)].
  
  Inductive Step: We must show P(k+1). That is, [state P(k+1)].
  [Derivation using P(k)]
  This completes the inductive step.
  
  By the Principle of Mathematical Induction, P(n) is true
  for all n ‚â• n‚ÇÄ. ‚ñ†
```

---

## üìù Summary Table

| Concept | Description |
|---------|-------------|
| Base Case | Verify $P(n_0)$ directly |
| Inductive Hypothesis | Assume $P(k)$ for arbitrary $k \geq n_0$ |
| Inductive Step | Prove $P(k) \Rightarrow P(k+1)$ |
| Result | $P(n)$ true for all $n \geq n_0$ |
| Analogy | Domino effect |
| Key requirement | Must USE the inductive hypothesis |
| Common uses | Sums, divisibility, inequalities |

---

## ‚ùì Quick Revision Questions

1. **Prove by induction: $\sum_{i=1}^{n} (2i - 1) = n^2$.**

2. **Prove: $n! > 2^n$ for all $n \geq 4$.**

3. **What goes wrong if we skip the base case?** Give an example of a false statement where the inductive step holds.

4. **Prove: $3 \mid (4^n - 1)$ for all $n \geq 1$.**

5. **Prove: $1 + 2 + 4 + \cdots + 2^n = 2^{n+1} - 1$.**

6. **Why is it essential to use the inductive hypothesis in the inductive step?**

---

[‚Üê Previous: Proof by Contradiction](03-proof-by-contradiction.md) | [Back to README](../README.md) | [Next: Strong Induction ‚Üí](05-strong-induction.md)
