# Chapter 4.2: Product to Sum Formulas

## Overview

Product to sum formulas allow us to convert **products** of trigonometric functions into **sums or differences**. These formulas are derived from the compound angle formulas and are useful for integration, simplifying expressions, and signal analysis.

---

## ğŸ“ The Product to Sum Formulas

### The Four Formulas

$$\boxed{\sin A \cos B = \frac{1}{2}[\sin(A + B) + \sin(A - B)]}$$

$$\boxed{\cos A \sin B = \frac{1}{2}[\sin(A + B) - \sin(A - B)]}$$

$$\boxed{\cos A \cos B = \frac{1}{2}[\cos(A + B) + \cos(A - B)]}$$

$$\boxed{\sin A \sin B = \frac{1}{2}[\cos(A - B) - \cos(A + B)]}$$

---

## ğŸ” Derivation of Product to Sum Formulas

### Deriving sin A cos B Formula

Start with the addition and subtraction formulas:
$$\sin(A + B) = \sin A \cos B + \cos A \sin B \quad \text{...(1)}$$
$$\sin(A - B) = \sin A \cos B - \cos A \sin B \quad \text{...(2)}$$

**Add equations (1) and (2):**
$$\sin(A + B) + \sin(A - B) = 2\sin A \cos B$$

$$\therefore \sin A \cos B = \frac{1}{2}[\sin(A + B) + \sin(A - B)]$$

### Deriving cos A sin B Formula

**Subtract equation (2) from (1):**
$$\sin(A + B) - \sin(A - B) = 2\cos A \sin B$$

$$\therefore \cos A \sin B = \frac{1}{2}[\sin(A + B) - \sin(A - B)]$$

### Deriving cos A cos B Formula

Start with:
$$\cos(A + B) = \cos A \cos B - \sin A \sin B \quad \text{...(3)}$$
$$\cos(A - B) = \cos A \cos B + \sin A \sin B \quad \text{...(4)}$$

**Add equations (3) and (4):**
$$\cos(A + B) + \cos(A - B) = 2\cos A \cos B$$

$$\therefore \cos A \cos B = \frac{1}{2}[\cos(A + B) + \cos(A - B)]$$

### Deriving sin A sin B Formula

**Subtract equation (3) from (4):**
$$\cos(A - B) - \cos(A + B) = 2\sin A \sin B$$

$$\therefore \sin A \sin B = \frac{1}{2}[\cos(A - B) - \cos(A + B)]$$

---

## ğŸ“Š Formula Reference Chart

```
    â”Œâ”€â”€â”€â”€â”€â”€â”€â”€â”€â”€â”€â”€â”€â”€â”€â”€â”€â”€â”€â”€â”€â”€â”€â”€â”€â”€â”€â”€â”€â”€â”€â”€â”€â”€â”€â”€â”€â”€â”€â”€â”€â”€â”€â”€â”€â”€â”€â”€â”€â”€â”€â”€â”€â”€â”€â”€â”€â”€â”€â”€â”€â”€â”€â”
    â”‚              PRODUCT TO SUM FORMULAS                          â”‚
    â”œâ”€â”€â”€â”€â”€â”€â”€â”€â”€â”€â”€â”€â”€â”€â”€â”€â”€â”€â”€â”€â”€â”€â”€â”€â”€â”€â”€â”€â”€â”€â”€â”€â”€â”€â”€â”€â”€â”€â”€â”€â”€â”€â”€â”€â”€â”€â”€â”€â”€â”€â”€â”€â”€â”€â”€â”€â”€â”€â”€â”€â”€â”€â”€â”¤
    â”‚                                                               â”‚
    â”‚  sin A cos B = Â½[sin(A+B) + sin(A-B)]     â†’ "sin + sin"      â”‚
    â”‚                                                               â”‚
    â”‚  cos A sin B = Â½[sin(A+B) - sin(A-B)]     â†’ "sin - sin"      â”‚
    â”‚                                                               â”‚
    â”‚  cos A cos B = Â½[cos(A+B) + cos(A-B)]     â†’ "cos + cos"      â”‚
    â”‚                                                               â”‚
    â”‚  sin A sin B = Â½[cos(A-B) - cos(A+B)]     â†’ "cos - cos"      â”‚
    â”‚                          â†‘       â†‘                            â”‚
    â”‚                      NOTE: Order reversed!                    â”‚
    â”‚                                                               â”‚
    â””â”€â”€â”€â”€â”€â”€â”€â”€â”€â”€â”€â”€â”€â”€â”€â”€â”€â”€â”€â”€â”€â”€â”€â”€â”€â”€â”€â”€â”€â”€â”€â”€â”€â”€â”€â”€â”€â”€â”€â”€â”€â”€â”€â”€â”€â”€â”€â”€â”€â”€â”€â”€â”€â”€â”€â”€â”€â”€â”€â”€â”€â”€â”€â”˜
```

---

## ğŸ§  Memory Techniques

### Pattern Recognition

```
    Product        â†’    Sum
    â”€â”€â”€â”€â”€â”€â”€â”€â”€           â”€â”€â”€â”€â”€â”€â”€
    sin Â· cos     â†’    sin Â± sin
    cos Â· sin     â†’    sin Â± sin
    cos Â· cos     â†’    cos + cos
    sin Â· sin     â†’    cos - cos (reversed order!)
```

### The "SCS Rule"

- **S**in Ã— **C**os = **S**in terms
- **C**os Ã— **C**os = **C**os terms (with +)
- **S**in Ã— **S**in = **C**os terms (with -, reversed)

---

## ğŸ§® Worked Examples

### Example 1: Basic Conversion

Express sin 5x cos 3x as a sum.

**Solution:**
Using sin A cos B = Â½[sin(A+B) + sin(A-B)]:
$$\sin 5x \cos 3x = \frac{1}{2}[\sin(5x + 3x) + \sin(5x - 3x)]$$
$$= \frac{1}{2}[\sin 8x + \sin 2x]$$
$$= \boxed{\frac{1}{2}\sin 8x + \frac{1}{2}\sin 2x}$$

### Example 2: cos Ã— cos Product

Express cos 4Î¸ cos 2Î¸ as a sum.

**Solution:**
Using cos A cos B = Â½[cos(A+B) + cos(A-B)]:
$$\cos 4\theta \cos 2\theta = \frac{1}{2}[\cos(4\theta + 2\theta) + \cos(4\theta - 2\theta)]$$
$$= \frac{1}{2}[\cos 6\theta + \cos 2\theta]$$
$$= \boxed{\frac{1}{2}\cos 6\theta + \frac{1}{2}\cos 2\theta}$$

### Example 3: sin Ã— sin Product

Express sin 3x sin x as a sum.

**Solution:**
Using sin A sin B = Â½[cos(A-B) - cos(A+B)]:
$$\sin 3x \sin x = \frac{1}{2}[\cos(3x - x) - \cos(3x + x)]$$
$$= \frac{1}{2}[\cos 2x - \cos 4x]$$
$$= \boxed{\frac{1}{2}\cos 2x - \frac{1}{2}\cos 4x}$$

### Example 4: Numerical Values

Find the exact value of sin 75Â° cos 15Â°.

**Solution:**
$$\sin 75Â° \cos 15Â° = \frac{1}{2}[\sin(75Â° + 15Â°) + \sin(75Â° - 15Â°)]$$
$$= \frac{1}{2}[\sin 90Â° + \sin 60Â°]$$
$$= \frac{1}{2}\left[1 + \frac{\sqrt{3}}{2}\right]$$
$$= \frac{1}{2} + \frac{\sqrt{3}}{4}$$
$$= \boxed{\frac{2 + \sqrt{3}}{4}}$$

### Example 5: cos Ã— sin Product

Express cos 7x sin 3x as a sum.

**Solution:**
Using cos A sin B = Â½[sin(A+B) - sin(A-B)]:
$$\cos 7x \sin 3x = \frac{1}{2}[\sin(7x + 3x) - \sin(7x - 3x)]$$
$$= \frac{1}{2}[\sin 10x - \sin 4x]$$
$$= \boxed{\frac{1}{2}\sin 10x - \frac{1}{2}\sin 4x}$$

### Example 6: Simplifying Complex Products

Simplify: 2 sin 50Â° cos 10Â°

**Solution:**
$$2 \sin 50Â° \cos 10Â° = 2 \cdot \frac{1}{2}[\sin(50Â° + 10Â°) + \sin(50Â° - 10Â°)]$$
$$= \sin 60Â° + \sin 40Â°$$
$$= \boxed{\frac{\sqrt{3}}{2} + \sin 40Â°}$$

---

## ğŸ“ Special Cases

### When A = B

$$\sin A \cos A = \frac{1}{2}[\sin 2A + \sin 0] = \frac{1}{2}\sin 2A$$

$$\cos A \cos A = \frac{1}{2}[\cos 2A + \cos 0] = \frac{1}{2}[\cos 2A + 1] = \frac{1 + \cos 2A}{2}$$

$$\sin A \sin A = \frac{1}{2}[\cos 0 - \cos 2A] = \frac{1}{2}[1 - \cos 2A] = \frac{1 - \cos 2A}{2}$$

These lead to the **power reduction formulas** (covered in Unit 5).

---

## ğŸ“Š Comparison Table

| Product Form | Sum Form |
|--------------|----------|
| sin A cos B | Â½[sin(A+B) + sin(A-B)] |
| cos A sin B | Â½[sin(A+B) - sin(A-B)] |
| cos A cos B | Â½[cos(A+B) + cos(A-B)] |
| sin A sin B | Â½[cos(A-B) - cos(A+B)] |

---

## ğŸ¯ Applications in Integration

### Why These Formulas Matter

Products of trigonometric functions are difficult to integrate directly. Converting to sums makes integration straightforward.

```
    âˆ« sin mx cos nx dx = âˆ« Â½[sin(m+n)x + sin(m-n)x] dx
    
    This is much easier to integrate!
```

**Example:**
$$\int \sin 3x \cos 2x \, dx = \int \frac{1}{2}[\sin 5x + \sin x] \, dx$$
$$= \frac{1}{2}\left[-\frac{\cos 5x}{5} - \cos x\right] + C$$
$$= -\frac{\cos 5x}{10} - \frac{\cos x}{2} + C$$

---

## ğŸ“ˆ Visualization

### Product vs Sum Representation

```
    Product: sin A cos B
    
    A wave (sin A) modulated by another wave (cos B)
    
        ~~~âˆ¿~~~âˆ¿~~~âˆ¿~~~âˆ¿~~~   Ã— 
        ___/â€¾â€¾â€¾\___/â€¾â€¾â€¾\___  
        ========================
        Complex combined pattern
    
    Sum: Â½[sin(A+B) + sin(A-B)]
    
        ~~~âˆ¿~~~âˆ¿~~~âˆ¿~~~âˆ¿~~~   +
        __âˆ¿__âˆ¿__âˆ¿__âˆ¿__âˆ¿__  
        ========================
        Sum of two simple waves
```

---

## ğŸŒ Real-World Applications

### 1. Signal Processing
Radio signals use product-to-sum conversions for modulation/demodulation.

### 2. Acoustics
Beat frequencies occur when two sound waves of slightly different frequencies combine.

### 3. Music Theory
Harmonic analysis of musical chords uses these formulas.

### 4. Electronics
Mixers in radio receivers multiply signals, then use these identities.

---

## ğŸ“‹ Summary Table

### Quick Reference

| If You Have | Use This Formula |
|-------------|------------------|
| sin Ã— cos | Â½[sin(sum) + sin(diff)] |
| cos Ã— sin | Â½[sin(sum) - sin(diff)] |
| cos Ã— cos | Â½[cos(sum) + cos(diff)] |
| sin Ã— sin | Â½[cos(diff) - cos(sum)] |

### Key Points to Remember

| Point | Detail |
|-------|--------|
| Factor of Â½ | Always present in result |
| sin Ã— cos â†’ sin | Product with different functions gives sin |
| cos Ã— cos â†’ cos | Same functions (cos) give cos |
| sin Ã— sin â†’ cos | Same functions (sin) give cos (reversed!) |
| Order matters for sin Ã— sin | It's cos(A-B) - cos(A+B), not the other way |

---

## â“ Quick Revision Questions

1. **Express sin 6x cos 2x as a sum.**

2. **Express cos 5Î¸ cos 3Î¸ as a sum.**

3. **Express sin 4x sin 2x as a sum.**

4. **Find the exact value of cos 75Â° cos 15Â°.**

5. **Prove that sin 3A cos A + cos 3A sin A = sin 4A using product formulas.**

6. **Why is the sin A sin B formula different from the others (reversed order)?**

<details>
<summary>Click to see answers</summary>

1. sin 6x cos 2x = Â½[sin 8x + sin 4x]

2. cos 5Î¸ cos 3Î¸ = Â½[cos 8Î¸ + cos 2Î¸]

3. sin 4x sin 2x = Â½[cos 2x - cos 6x]

4. cos 75Â° cos 15Â° = Â½[cos 90Â° + cos 60Â°]  
   = Â½[0 + Â½] = **1/4**

5. LHS = sin 3A cos A + cos 3A sin A  
   = sin(3A + A) [using addition formula]  
   = sin 4A = RHS âœ“  
   (Note: This is actually the addition formula directly!)

6. When deriving from cos(A-B) - cos(A+B) = 2 sin A sin B, the subtraction of cosines naturally gives cos(A-B) first. The negative sign attaches to cos(A+B), resulting in the reversed order.

</details>

---

## Navigation

| Previous | Up | Next |
|----------|-------|------|
| [â† 4.1 Addition Formulas](01-addition-formulas.md) | [Unit 4 Index](README.md) | [4.3 Sum to Product â†’](03-sum-to-product.md) |

---

[â† Back to Main Index](../README.md)
