# Chapter 4.4: Applications of Compound Angle Formulas

## Overview

This chapter consolidates all compound angle formulas and demonstrates their practical applications in solving problems, proving identities, and working with real-world scenarios involving waves, physics, and engineering.

---

## ğŸ“‹ Complete Formula Reference

### Addition and Subtraction Formulas

| Formula Type | Expression |
|--------------|------------|
| sin(A + B) | sin A cos B + cos A sin B |
| sin(A - B) | sin A cos B - cos A sin B |
| cos(A + B) | cos A cos B - sin A sin B |
| cos(A - B) | cos A cos B + sin A sin B |
| tan(A + B) | (tan A + tan B)/(1 - tan A tan B) |
| tan(A - B) | (tan A - tan B)/(1 + tan A tan B) |

### Product to Sum Formulas

| Product | Sum/Difference |
|---------|----------------|
| 2 sin A cos B | sin(A+B) + sin(A-B) |
| 2 cos A sin B | sin(A+B) - sin(A-B) |
| 2 cos A cos B | cos(A+B) + cos(A-B) |
| 2 sin A sin B | cos(A-B) - cos(A+B) |

### Sum to Product Formulas

| Sum/Difference | Product |
|----------------|---------|
| sin A + sin B | 2 sin((A+B)/2) cos((A-B)/2) |
| sin A - sin B | 2 cos((A+B)/2) sin((A-B)/2) |
| cos A + cos B | 2 cos((A+B)/2) cos((A-B)/2) |
| cos A - cos B | -2 sin((A+B)/2) sin((A-B)/2) |

---

## ğŸ“ Application Type 1: Finding Exact Values

### Standard Technique

```
    For angles like 15Â°, 75Â°, 105Â°, 165Â°, etc.
    
    Express as sum/difference of standard angles:
    â”Œâ”€â”€â”€â”€â”€â”€â”€â”€â”€â”€â”€â”€â”€â”€â”€â”€â”€â”€â”€â”€â”€â”€â”€â”€â”€â”€â”€â”€â”€â”€â”€â”€â”€â”€â”€â”€â”€â”€â”€â”€â”€â”
    â”‚  15Â° = 45Â° - 30Â° = 60Â° - 45Â°           â”‚
    â”‚  75Â° = 45Â° + 30Â° = 120Â° - 45Â°          â”‚
    â”‚  105Â° = 60Â° + 45Â° = 180Â° - 75Â°         â”‚
    â”‚  165Â° = 180Â° - 15Â° = 120Â° + 45Â°        â”‚
    â””â”€â”€â”€â”€â”€â”€â”€â”€â”€â”€â”€â”€â”€â”€â”€â”€â”€â”€â”€â”€â”€â”€â”€â”€â”€â”€â”€â”€â”€â”€â”€â”€â”€â”€â”€â”€â”€â”€â”€â”€â”€â”˜
```

### Example 1: Find sin 15Â°

**Solution:**
$$\sin 15Â° = \sin(45Â° - 30Â°)$$
$$= \sin 45Â° \cos 30Â° - \cos 45Â° \sin 30Â°$$
$$= \frac{\sqrt{2}}{2} \cdot \frac{\sqrt{3}}{2} - \frac{\sqrt{2}}{2} \cdot \frac{1}{2}$$
$$= \frac{\sqrt{6}}{4} - \frac{\sqrt{2}}{4}$$
$$= \boxed{\frac{\sqrt{6} - \sqrt{2}}{4}}$$

### Example 2: Find tan 75Â°

**Solution:**
$$\tan 75Â° = \tan(45Â° + 30Â°)$$
$$= \frac{\tan 45Â° + \tan 30Â°}{1 - \tan 45Â° \tan 30Â°}$$
$$= \frac{1 + \frac{1}{\sqrt{3}}}{1 - 1 \cdot \frac{1}{\sqrt{3}}}$$
$$= \frac{\sqrt{3} + 1}{\sqrt{3} - 1}$$

Rationalizing:
$$= \frac{(\sqrt{3} + 1)^2}{(\sqrt{3} - 1)(\sqrt{3} + 1)}$$
$$= \frac{3 + 2\sqrt{3} + 1}{3 - 1}$$
$$= \frac{4 + 2\sqrt{3}}{2}$$
$$= \boxed{2 + \sqrt{3}}$$

### Example 3: Find cos 105Â°

**Solution:**
$$\cos 105Â° = \cos(60Â° + 45Â°)$$
$$= \cos 60Â° \cos 45Â° - \sin 60Â° \sin 45Â°$$
$$= \frac{1}{2} \cdot \frac{\sqrt{2}}{2} - \frac{\sqrt{3}}{2} \cdot \frac{\sqrt{2}}{2}$$
$$= \frac{\sqrt{2}}{4} - \frac{\sqrt{6}}{4}$$
$$= \boxed{\frac{\sqrt{2} - \sqrt{6}}{4}}$$

---

## ğŸ“ Application Type 2: Proving Identities

### Strategy for Proving Identities

```
    â”Œâ”€â”€â”€â”€â”€â”€â”€â”€â”€â”€â”€â”€â”€â”€â”€â”€â”€â”€â”€â”€â”€â”€â”€â”€â”€â”€â”€â”€â”€â”€â”€â”€â”€â”€â”€â”€â”€â”€â”€â”€â”€â”€â”€â”€â”€â”€â”€â”€â”€â”€â”€â”€â”€â”€â”€â”€â”€â”
    â”‚                  IDENTITY PROOF STRATEGY                â”‚
    â”œâ”€â”€â”€â”€â”€â”€â”€â”€â”€â”€â”€â”€â”€â”€â”€â”€â”€â”€â”€â”€â”€â”€â”€â”€â”€â”€â”€â”€â”€â”€â”€â”€â”€â”€â”€â”€â”€â”€â”€â”€â”€â”€â”€â”€â”€â”€â”€â”€â”€â”€â”€â”€â”€â”€â”€â”€â”€â”¤
    â”‚  1. Work with the more complex side                     â”‚
    â”‚  2. Apply compound angle formulas                       â”‚
    â”‚  3. Use sum/product transformations if needed           â”‚
    â”‚  4. Simplify using fundamental identities               â”‚
    â”‚  5. Arrive at the simpler side                         â”‚
    â””â”€â”€â”€â”€â”€â”€â”€â”€â”€â”€â”€â”€â”€â”€â”€â”€â”€â”€â”€â”€â”€â”€â”€â”€â”€â”€â”€â”€â”€â”€â”€â”€â”€â”€â”€â”€â”€â”€â”€â”€â”€â”€â”€â”€â”€â”€â”€â”€â”€â”€â”€â”€â”€â”€â”€â”€â”€â”˜
```

### Example 4: Prove sin(A+B) sin(A-B) = sinÂ²A - sinÂ²B

**Solution:**
$$\text{LHS} = \sin(A+B) \cdot \sin(A-B)$$
$$= (\sin A \cos B + \cos A \sin B)(\sin A \cos B - \cos A \sin B)$$

Using (x + y)(x - y) = xÂ² - yÂ²:
$$= \sin^2 A \cos^2 B - \cos^2 A \sin^2 B$$
$$= \sin^2 A (1 - \sin^2 B) - (1 - \sin^2 A) \sin^2 B$$
$$= \sin^2 A - \sin^2 A \sin^2 B - \sin^2 B + \sin^2 A \sin^2 B$$
$$= \sin^2 A - \sin^2 B = \text{RHS} \quad \checkmark$$

### Example 5: Prove cos(A+B) cos(A-B) = cosÂ²A - sinÂ²B

**Solution:**
$$\text{LHS} = \cos(A+B) \cdot \cos(A-B)$$
$$= (\cos A \cos B - \sin A \sin B)(\cos A \cos B + \sin A \sin B)$$
$$= \cos^2 A \cos^2 B - \sin^2 A \sin^2 B$$
$$= \cos^2 A (1 - \sin^2 B) - (1 - \cos^2 A) \sin^2 B$$
$$= \cos^2 A - \cos^2 A \sin^2 B - \sin^2 B + \cos^2 A \sin^2 B$$
$$= \cos^2 A - \sin^2 B = \text{RHS} \quad \checkmark$$

### Example 6: Prove tan(45Â° + A) Â· tan(45Â° - A) = 1

**Solution:**
$$\text{LHS} = \tan(45Â° + A) \cdot \tan(45Â° - A)$$
$$= \frac{1 + \tan A}{1 - \tan A} \cdot \frac{1 - \tan A}{1 + \tan A}$$
$$= \frac{(1 + \tan A)(1 - \tan A)}{(1 - \tan A)(1 + \tan A)}$$
$$= 1 = \text{RHS} \quad \checkmark$$

---

## ğŸ“ Application Type 3: Solving Equations

### Example 7: Solve sin x + sin 3x = 0

**Solution:**
Using sum to product formula:
$$2\sin\left(\frac{x + 3x}{2}\right)\cos\left(\frac{x - 3x}{2}\right) = 0$$
$$2\sin 2x \cos(-x) = 0$$
$$2\sin 2x \cos x = 0$$

Either sin 2x = 0 or cos x = 0

**Case 1:** sin 2x = 0
$$2x = n\pi, \quad n \in \mathbb{Z}$$
$$x = \frac{n\pi}{2}$$

**Case 2:** cos x = 0
$$x = \frac{\pi}{2} + n\pi = \frac{(2n+1)\pi}{2}$$

Combining: $$\boxed{x = \frac{n\pi}{2}, \quad n \in \mathbb{Z}}$$

### Example 8: Solve cos 5x + cos 3x = 0

**Solution:**
Using sum to product:
$$2\cos\left(\frac{5x + 3x}{2}\right)\cos\left(\frac{5x - 3x}{2}\right) = 0$$
$$2\cos 4x \cos x = 0$$

Either cos 4x = 0 or cos x = 0

**Case 1:** cos 4x = 0
$$4x = \frac{\pi}{2} + n\pi$$
$$x = \frac{\pi}{8} + \frac{n\pi}{4} = \frac{(2n+1)\pi}{8}$$

**Case 2:** cos x = 0
$$x = \frac{(2n+1)\pi}{2}$$

---

## ğŸ“ Application Type 4: Wave Combination

### Combining Sinusoidal Functions

When we have expressions of the form:
$$a\sin\theta + b\cos\theta$$

We can write it as:
$$R\sin(\theta + \phi)$$

where $R = \sqrt{a^2 + b^2}$ and $\tan\phi = \frac{b}{a}$

```
    â”Œâ”€â”€â”€â”€â”€â”€â”€â”€â”€â”€â”€â”€â”€â”€â”€â”€â”€â”€â”€â”€â”€â”€â”€â”€â”€â”€â”€â”€â”€â”€â”€â”€â”€â”€â”€â”€â”€â”€â”€â”€â”€â”€â”€â”€â”€â”€â”€â”€â”€â”€â”€â”€â”€â”€â”€â”€â”€â”€â”€â”€â”
    â”‚         CONVERSION: a sin Î¸ + b cos Î¸ = R sin(Î¸ + Ï†)       â”‚
    â”œâ”€â”€â”€â”€â”€â”€â”€â”€â”€â”€â”€â”€â”€â”€â”€â”€â”€â”€â”€â”€â”€â”€â”€â”€â”€â”€â”€â”€â”€â”€â”€â”€â”€â”€â”€â”€â”€â”€â”€â”€â”€â”€â”€â”€â”€â”€â”€â”€â”€â”€â”€â”€â”€â”€â”€â”€â”€â”€â”€â”€â”¤
    â”‚                                                            â”‚
    â”‚             R = âˆš(aÂ² + bÂ²)                                 â”‚
    â”‚                                                            â”‚
    â”‚             tan Ï† = b/a                                    â”‚
    â”‚                                                            â”‚
    â”‚   Alternative: R cos(Î¸ - Ïˆ) where tan Ïˆ = a/b             â”‚
    â”‚                                                            â”‚
    â””â”€â”€â”€â”€â”€â”€â”€â”€â”€â”€â”€â”€â”€â”€â”€â”€â”€â”€â”€â”€â”€â”€â”€â”€â”€â”€â”€â”€â”€â”€â”€â”€â”€â”€â”€â”€â”€â”€â”€â”€â”€â”€â”€â”€â”€â”€â”€â”€â”€â”€â”€â”€â”€â”€â”€â”€â”€â”€â”€â”€â”˜
```

### Example 9: Express 3sin Î¸ + 4cos Î¸ in the form R sin(Î¸ + Ï†)

**Solution:**
$$R = \sqrt{3^2 + 4^2} = \sqrt{9 + 16} = \sqrt{25} = 5$$

$$\tan\phi = \frac{4}{3}$$
$$\phi = \tan^{-1}\left(\frac{4}{3}\right) \approx 53.13Â°$$

$$\therefore 3\sin\theta + 4\cos\theta = 5\sin(\theta + 53.13Â°)$$

**Verification:**
$$5\sin(\theta + \phi) = 5(\sin\theta\cos\phi + \cos\theta\sin\phi)$$
$$= 5\sin\theta \cdot \frac{3}{5} + 5\cos\theta \cdot \frac{4}{5}$$
$$= 3\sin\theta + 4\cos\theta \quad \checkmark$$

### Example 10: Find maximum value of 5sin x + 12cos x

**Solution:**
$$R = \sqrt{5^2 + 12^2} = \sqrt{25 + 144} = \sqrt{169} = 13$$

Since the maximum value of sin(x + Ï†) is 1:

**Maximum value = 13**
**Minimum value = -13**

---

## ğŸ“ Application Type 5: Physics Applications

### Simple Harmonic Motion

```
    Superposition of Two SHM Waves:
    
    yâ‚ = A sin(Ï‰t)
    yâ‚‚ = A sin(Ï‰t + Ï†)
    
    Combined: y = yâ‚ + yâ‚‚ = 2A cos(Ï†/2) sin(Ï‰t + Ï†/2)
    
    â”Œâ”€â”€â”€â”€â”€â”€â”€â”€â”€â”€â”€â”€â”€â”€â”€â”€â”€â”€â”€â”€â”€â”€â”€â”€â”€â”€â”€â”€â”€â”€â”€â”€â”€â”€â”€â”€â”€â”€â”€â”€â”€â”€â”€â”€â”€â”
    â”‚     Resultant amplitude = 2A cos(Ï†/2)       â”‚
    â”‚     Phase shift = Ï†/2                       â”‚
    â””â”€â”€â”€â”€â”€â”€â”€â”€â”€â”€â”€â”€â”€â”€â”€â”€â”€â”€â”€â”€â”€â”€â”€â”€â”€â”€â”€â”€â”€â”€â”€â”€â”€â”€â”€â”€â”€â”€â”€â”€â”€â”€â”€â”€â”€â”˜
```

### Example 11: Superposition of Waves

Two sound waves are given by yâ‚ = 5sin(100Ï€t) and yâ‚‚ = 5sin(100Ï€t + Ï€/3).
Find the resultant wave.

**Solution:**
$$y = y_1 + y_2 = 5\sin(100\pi t) + 5\sin(100\pi t + \frac{\pi}{3})$$

Using sum to product with A = 100Ï€t + Ï€/3 and B = 100Ï€t:
$$= 2 \cdot 5 \cdot \sin\left(\frac{(100\pi t + \frac{\pi}{3}) + 100\pi t}{2}\right)\cos\left(\frac{(100\pi t + \frac{\pi}{3}) - 100\pi t}{2}\right)$$
$$= 10\sin\left(100\pi t + \frac{\pi}{6}\right)\cos\left(\frac{\pi}{6}\right)$$
$$= 10 \cdot \frac{\sqrt{3}}{2} \cdot \sin\left(100\pi t + \frac{\pi}{6}\right)$$
$$= 5\sqrt{3}\sin\left(100\pi t + \frac{\pi}{6}\right)$$

**Resultant amplitude = 5âˆš3 â‰ˆ 8.66**

---

## ğŸ“Š Problem-Solving Flowchart

```
    â”Œâ”€â”€â”€â”€â”€â”€â”€â”€â”€â”€â”€â”€â”€â”€â”€â”€â”€â”€â”€â”€â”€â”€â”€â”€â”€â”€â”€â”€â”€â”€â”€â”€â”€â”€â”€â”€â”€â”€â”€â”€â”€â”€â”€â”€â”€â”€â”€â”€â”€â”€â”€â”€â”€â”€â”€â”€â”€â”€â”€â”€â”€â”
    â”‚                 COMPOUND ANGLE PROBLEM                      â”‚
    â””â”€â”€â”€â”€â”€â”€â”€â”€â”€â”€â”€â”€â”€â”€â”€â”€â”€â”€â”€â”€â”€â”€â”€â”€â”¬â”€â”€â”€â”€â”€â”€â”€â”€â”€â”€â”€â”€â”€â”€â”€â”€â”€â”€â”€â”€â”€â”€â”€â”€â”€â”€â”€â”€â”€â”€â”€â”€â”€â”€â”€â”€â”˜
                             â†“
              â”Œâ”€â”€â”€â”€â”€â”€â”€â”€â”€â”€â”€â”€â”€â”€â”´â”€â”€â”€â”€â”€â”€â”€â”€â”€â”€â”€â”€â”€â”€â”
              â”‚   What type of problem?     â”‚
              â””â”€â”€â”€â”€â”€â”€â”€â”€â”€â”€â”€â”€â”€â”€â”¬â”€â”€â”€â”€â”€â”€â”€â”€â”€â”€â”€â”€â”€â”€â”˜
                             â”‚
        â”Œâ”€â”€â”€â”€â”€â”€â”€â”€â”€â”€â”€â”€â”¬â”€â”€â”€â”€â”€â”€â”€â”´â”€â”€â”€â”€â”€â”€â”€â”¬â”€â”€â”€â”€â”€â”€â”€â”€â”€â”€â”€â”€â”
        â†“            â†“               â†“            â†“
    â”Œâ”€â”€â”€â”€â”€â”€â”€â”   â”Œâ”€â”€â”€â”€â”€â”€â”€â”€â”€â”   â”Œâ”€â”€â”€â”€â”€â”€â”€â”€â”€â”€â”   â”Œâ”€â”€â”€â”€â”€â”€â”€â”€â”€â”
    â”‚ Exact â”‚   â”‚ Prove   â”‚   â”‚  Solve   â”‚   â”‚Combine  â”‚
    â”‚ Value â”‚   â”‚Identity â”‚   â”‚ Equation â”‚   â”‚ Waves   â”‚
    â””â”€â”€â”€â”¬â”€â”€â”€â”˜   â””â”€â”€â”€â”€â”¬â”€â”€â”€â”€â”˜   â””â”€â”€â”€â”€â”¬â”€â”€â”€â”€â”€â”˜   â””â”€â”€â”€â”€â”¬â”€â”€â”€â”€â”˜
        â†“            â†“             â†“              â†“
    Express as    Work with     Convert to     Find R and
    sum/diff of   complex       product        Ï† for
    standard      side first    form           R sin(Î¸+Ï†)
    angles
```

---

## ğŸ“ Advanced Identities

### Triple Combination

$$\sin(A + B + C) = \sin A \cos B \cos C + \cos A \sin B \cos C$$
$$\quad\quad\quad\quad\quad\quad + \cos A \cos B \sin C - \sin A \sin B \sin C$$

Or equivalently:
$$\sin(A + B + C) = \sum\sin A \cos B \cos C - \sin A \sin B \sin C$$

### Tangent of Sum of Three Angles

$$\tan(A + B + C) = \frac{\tan A + \tan B + \tan C - \tan A \tan B \tan C}{1 - \tan A \tan B - \tan B \tan C - \tan C \tan A}$$

---

## ğŸ¯ Important Special Results

### When A + B = 45Â°

$$\tan(A + B) = 1$$
$$\frac{\tan A + \tan B}{1 - \tan A \tan B} = 1$$
$$\tan A + \tan B = 1 - \tan A \tan B$$
$$\boxed{(1 + \tan A)(1 + \tan B) = 2}$$

### When A + B = 90Â°

$$\sin(A + B) = 1, \quad \cos(A + B) = 0$$
$$\sin A = \cos B, \quad \cos A = \sin B$$
$$\tan A \tan B = 1$$

### When A + B = 180Â°

$$\sin A = \sin B, \quad \cos A = -\cos B$$
$$\tan A = -\tan B$$

---

## ğŸ“‹ Summary Table

### Application Types and Techniques

| Application | Technique | Key Formula(s) |
|-------------|-----------|----------------|
| Exact values | Express as sum/diff of standard angles | sin(AÂ±B), cos(AÂ±B), tan(AÂ±B) |
| Proving identities | Expand using compound formulas | All compound angle formulas |
| Solving equations | Convert sum to product | Sum to product formulas |
| Combining waves | Express as R sin(Î¸ + Ï†) | R = âˆš(aÂ² + bÂ²), tan Ï† = b/a |
| Physics problems | Superposition of waves | All formulas as needed |

### Key Values to Remember

| Expression | Exact Value |
|------------|-------------|
| sin 15Â° | (âˆš6 - âˆš2)/4 |
| cos 15Â° | (âˆš6 + âˆš2)/4 |
| tan 15Â° | 2 - âˆš3 |
| sin 75Â° | (âˆš6 + âˆš2)/4 |
| cos 75Â° | (âˆš6 - âˆš2)/4 |
| tan 75Â° | 2 + âˆš3 |

---

## â“ Quick Revision Questions

1. **Find the exact value of sin 105Â° + cos 105Â°.**

2. **Prove that: tan 3A - tan 2A - tan A = tan 3A tan 2A tan A**

3. **Express 5 sin Î¸ - 12 cos Î¸ in the form R sin(Î¸ - Ï†). Find R and Ï†.**

4. **Solve: sin 5x - sin x = sin 3x for x âˆˆ [0, 2Ï€]**

5. **If A + B = 45Â°, prove that (1 + tan A)(1 + tan B) = 2**

6. **Two waves yâ‚ = 3sin(Ï‰t) and yâ‚‚ = 4cos(Ï‰t) are superposed. Find the amplitude of the resultant wave.**

<details>
<summary>Click to see answers</summary>

1. sin 105Â° + cos 105Â°  
   = sin(60Â°+45Â°) + cos(60Â°+45Â°)  
   = (sin60Â°cos45Â° + cos60Â°sin45Â°) + (cos60Â°cos45Â° - sin60Â°sin45Â°)  
   = (âˆš3/2)(âˆš2/2) + (1/2)(âˆš2/2) + (1/2)(âˆš2/2) - (âˆš3/2)(âˆš2/2)  
   = âˆš6/4 + âˆš2/4 + âˆš2/4 - âˆš6/4  
   = **âˆš2/2**

2. Since 3A = 2A + A:
   tan 3A = tan(2A + A) = (tan 2A + tan A)/(1 - tan 2A tan A)  
   tan 3A(1 - tan 2A tan A) = tan 2A + tan A  
   tan 3A - tan 3A tan 2A tan A = tan 2A + tan A  
   **tan 3A - tan 2A - tan A = tan 3A tan 2A tan A** âœ“

3. R = âˆš(5Â² + 12Â²) = âˆš(25 + 144) = **13**  
   For R sin(Î¸ - Ï†) = R(sin Î¸ cos Ï† - cos Î¸ sin Ï†)  
   Comparing: R cos Ï† = 5 and R sin Ï† = 12  
   tan Ï† = 12/5  
   **Ï† = tanâ»Â¹(12/5) â‰ˆ 67.38Â°**

4. sin 5x - sin x = sin 3x  
   2 cos 3x sin 2x = sin 3x  
   2 cos 3x sin 2x - sin 3x = 0  
   sin 3x(2 cos 3x Â· (sin 2x/sin 3x) - 1) = 0  
   
   Actually, rearranging:  
   2 cos 3x sin 2x = sin 3x  
   If sin 3x â‰  0: 2 cos 3x sin 2x = sin 3x  
   Using sin 3x = sin 2x cos x + cos 2x sin x... (complex)  
   
   Simpler: sin 5x - sin 3x = sin x  
   2 cos 4x sin x = sin x  
   sin x(2 cos 4x - 1) = 0  
   sin x = 0 â†’ x = 0, Ï€, 2Ï€  
   cos 4x = 1/2 â†’ 4x = Ï€/3, 5Ï€/3, 7Ï€/3, 11Ï€/3, 13Ï€/3, 17Ï€/3, 19Ï€/3, 23Ï€/3  
   x = **Ï€/12, 5Ï€/12, 7Ï€/12, 11Ï€/12, 13Ï€/12, 17Ï€/12, 19Ï€/12, 23Ï€/12, 0, Ï€, 2Ï€**

5. A + B = 45Â°, so tan(A + B) = 1  
   (tan A + tan B)/(1 - tan A tan B) = 1  
   tan A + tan B = 1 - tan A tan B  
   1 + tan A + tan B + tan A tan B = 2  
   (1 + tan A) + tan B(1 + tan A) = 2  
   **(1 + tan A)(1 + tan B) = 2** âœ“

6. y = 3 sin(Ï‰t) + 4 cos(Ï‰t) = 3 sin(Ï‰t) + 4 sin(Ï‰t + Ï€/2)  
   R = âˆš(3Â² + 4Â²) = âˆš25 = **5**  
   The resultant amplitude is **5**.

</details>

---

## Navigation

| Previous | Up | Next |
|----------|-------|------|
| [â† 4.3 Sum to Product](03-sum-to-product.md) | [Unit 4 Index](README.md) | [Unit 5: Multiple Angles â†’](../05-Multiple-Submultiple-Angles/README.md) |

---

[â† Back to Main Index](../README.md)
