# Chapter 7.4: Generating Functions for Recurrences

[â† Previous: Non-Homogeneous Recurrence](03-non-homogeneous-recurrence.md) | [Back to README](../README.md) | [Next: Solving Recurrences â†’](05-solving-recurrences.md)

---

## ğŸ“‹ Chapter Overview

Generating functions provide a **universal method** for solving linear recurrences â€” both homogeneous and non-homogeneous. Instead of guessing solution forms, we transform the recurrence into an algebraic equation, solve it, and extract the coefficients.

---

## 1. The GF Method â€” Step by Step

```
  â”Œâ”€â”€â”€â”€â”€â”€â”€â”€â”€â”€â”€â”€â”€â”€â”€â”€â”€â”€â”€â”€â”€â”€â”€â”€â”€â”€â”€â”€â”€â”€â”€â”€â”€â”€â”€â”€â”€â”€â”€â”€â”€â”€â”€â”€â”€â”€â”€â”€â”€â”€â”
  â”‚  Generating Function Method for Recurrences       â”‚
  â”‚                                                    â”‚
  â”‚  1. Define G(x) = Î£ aâ‚™ xâ¿                        â”‚
  â”‚  2. Multiply both sides of recurrence by xâ¿       â”‚
  â”‚  3. Sum over all valid n                           â”‚
  â”‚  4. Express sums in terms of G(x)                 â”‚
  â”‚  5. Solve algebraically for G(x)                  â”‚
  â”‚  6. Decompose G(x) using partial fractions        â”‚
  â”‚  7. Extract [xâ¿] = aâ‚™ (the coefficient of xâ¿)    â”‚
  â””â”€â”€â”€â”€â”€â”€â”€â”€â”€â”€â”€â”€â”€â”€â”€â”€â”€â”€â”€â”€â”€â”€â”€â”€â”€â”€â”€â”€â”€â”€â”€â”€â”€â”€â”€â”€â”€â”€â”€â”€â”€â”€â”€â”€â”€â”€â”€â”€â”€â”€â”˜
```

### Key identities for step 4:

$$\sum_{n=1}^{\infty} a_{n-1} x^n = x \cdot G(x)$$

$$\sum_{n=2}^{\infty} a_{n-2} x^n = x^2 \cdot G(x)$$

$$\sum_{n=0}^{\infty} a_n x^n = G(x)$$

---

## 2. Example: First-Order Recurrence

Solve $a_n = 3a_{n-1} + 2$, $a_0 = 1$.

**Step 1.** $G(x) = \sum_{n=0}^{\infty} a_n x^n$

**Step 2-3.** Multiply by $x^n$ and sum for $n \geq 1$:

$$\sum_{n=1}^{\infty} a_n x^n = 3\sum_{n=1}^{\infty} a_{n-1} x^n + \sum_{n=1}^{\infty} 2x^n$$

$$G(x) - a_0 = 3x \cdot G(x) + \frac{2x}{1-x}$$

**Step 4-5.** $G(x)(1-3x) = 1 + \frac{2x}{1-x}$

$$G(x) = \frac{1}{1-3x} + \frac{2x}{(1-x)(1-3x)}$$

**Partial fractions** on second term: $\frac{2x}{(1-x)(1-3x)} = \frac{-1}{1-x} + \frac{1}{1-3x}$

$$G(x) = \frac{2}{1-3x} - \frac{1}{1-x}$$

**Step 6-7.** Extract coefficients:

$$a_n = 2 \cdot 3^n - 1$$

**Verify:** $a_0 = 2-1 = 1$ âœ“, $a_1 = 6-1 = 5 = 3(1)+2$ âœ“

---

## 3. Example: Fibonacci Numbers

$F_n = F_{n-1} + F_{n-2}$, $F_0 = 0, F_1 = 1$.

Let $G(x) = \sum_{n=0}^{\infty} F_n x^n$.

For $n \geq 2$: multiply recurrence by $x^n$ and sum:

$$G(x) - F_0 - F_1 x = x(G(x) - F_0) + x^2 G(x)$$

$$G(x) - x = xG(x) + x^2 G(x)$$

$$G(x)(1 - x - x^2) = x$$

$$G(x) = \frac{x}{1-x-x^2}$$

**Partial fractions:** Factor $1-x-x^2 = -(x-\phi^{-1})(x-\hat\phi^{-1})$ where $\phi = \frac{1+\sqrt{5}}{2}$.

$$G(x) = \frac{1}{\sqrt{5}}\left(\frac{1}{1-\phi x} - \frac{1}{1-\hat\phi x}\right)$$

$$F_n = [x^n]G(x) = \frac{1}{\sqrt{5}}(\phi^n - \hat\phi^n)$$

This matches **Binet's formula**.

---

## 4. Example: Non-Homogeneous with Exponential

Solve $a_n = 2a_{n-1} + 2^n$, $a_0 = 0$.

$G(x) - 0 = 2x \cdot G(x) + \sum_{n=1}^{\infty} 2^n x^n = 2xG(x) + \frac{2x}{1-2x}$

$$G(x)(1-2x) = \frac{2x}{1-2x}$$

$$G(x) = \frac{2x}{(1-2x)^2}$$

Using the identity $\frac{1}{(1-cx)^2} = \sum_{n=0}^{\infty} (n+1)c^n x^n$:

$$\frac{2x}{(1-2x)^2} = \sum_{n=1}^{\infty} n \cdot 2^n x^n$$

$$\boxed{a_n = n \cdot 2^n}$$

---

## 5. Partial Fraction Decomposition

This is the critical algebraic step. Common cases:

### Distinct Linear Factors

$$\frac{P(x)}{(1-ax)(1-bx)} = \frac{A}{1-ax} + \frac{B}{1-bx}$$

Extract: $[x^n] = A \cdot a^n + B \cdot b^n$

### Repeated Linear Factor

$$\frac{P(x)}{(1-ax)^2} = \frac{A}{1-ax} + \frac{B}{(1-ax)^2}$$

Using $[x^n]\frac{1}{(1-ax)^k} = \binom{n+k-1}{k-1}a^n$:

$$[x^n] = A \cdot a^n + B(n+1) \cdot a^n$$

### Quick Reference

| GF Term | Coefficient of $x^n$ |
|---------|:--------------------:|
| $\frac{1}{1-ax}$ | $a^n$ |
| $\frac{1}{(1-ax)^2}$ | $(n+1)a^n$ |
| $\frac{1}{(1-ax)^3}$ | $\binom{n+2}{2}a^n$ |
| $\frac{x}{(1-ax)^2}$ | $na^{n-1}$ |

---

## 6. Catalan Numbers via GFs

The Catalan numbers satisfy: $C_n = \sum_{k=0}^{n-1} C_k C_{n-1-k}$, $C_0 = 1$.

Let $G(x) = \sum C_n x^n$. The convolution sum means:

$$G(x) = 1 + x \cdot G(x)^2$$

This is a **quadratic** in $G(x)$:

$$xG^2 - G + 1 = 0 \implies G(x) = \frac{1 - \sqrt{1-4x}}{2x}$$

Using the generalized binomial theorem:

$$C_n = [x^n]G(x) = \frac{1}{n+1}\binom{2n}{n}$$

---

## 7. Advantages and Limitations

| Aspect | GF Method |
|--------|-----------|
| Universality | Works for any linear recurrence |
| Non-linear | Can handle some (e.g., Catalan) |
| Difficulty | Partial fractions can be tedious |
| When to use | When undetermined coefficients fails, or for complicated $f(n)$ |
| Alternative | Characteristic equation is faster for simple cases |

---

## 8. Real-World Applications

```
  â”Œâ”€â”€â”€â”€â”€â”€â”€â”€â”€â”€â”€â”€â”€â”€â”€â”€â”€â”€â”€â”€â”€â”€â”€â”€â”€â”€â”€â”€â”€â”€â”€â”€â”€â”€â”€â”€â”€â”€â”€â”€â”€â”€â”€â”€â”€â”€â”€â”
  â”‚       Generating Functions in Practice         â”‚
  â”‚                                                â”‚
  â”‚  1. Probability                                â”‚
  â”‚     GF of PMF = probability generating         â”‚
  â”‚     function â†’ E[X] = G'(1)                    â”‚
  â”‚                                                â”‚
  â”‚  2. Queueing Theory                            â”‚
  â”‚     Steady-state distributions via GFs          â”‚
  â”‚                                                â”‚
  â”‚  3. Enumeration                                â”‚
  â”‚     Lattice paths, partitions, tilings          â”‚
  â”‚                                                â”‚
  â”‚  4. Compiler Design                            â”‚
  â”‚     Ambiguity in grammars analyzed via GFs      â”‚
  â””â”€â”€â”€â”€â”€â”€â”€â”€â”€â”€â”€â”€â”€â”€â”€â”€â”€â”€â”€â”€â”€â”€â”€â”€â”€â”€â”€â”€â”€â”€â”€â”€â”€â”€â”€â”€â”€â”€â”€â”€â”€â”€â”€â”€â”€â”€â”€â”˜
```

---

## ğŸ“ Summary Table

| Concept | Description |
|---------|-------------|
| $G(x) = \sum a_n x^n$ | Define generating function |
| Shift: $a_{n-1}$ â†’ $xG(x)$ | Right-shift by multiplication |
| Solve algebraically | Get $G(x) = \text{rational function}$ |
| Partial fractions | Decompose into simple terms |
| Extract $[x^n]$ | Read off closed-form for $a_n$ |

---

## â“ Quick Revision Questions

1. **Use GFs to solve $a_n = a_{n-1} + 1$, $a_0 = 0$.**

2. **Find the GF for the recurrence $a_n = 3a_{n-1}$, $a_0 = 2$. What is the closed form?**

3. **What is $[x^n]\frac{1}{(1-2x)^2}$?**

4. **How does the shift $a_{n-2}$ translate in GF terms?**

5. **Use GFs to derive the closed form for the Tower of Hanoi recurrence: $T_n = 2T_{n-1}+1$, $T_0 = 0$.**

---

[â† Previous: Non-Homogeneous Recurrence](03-non-homogeneous-recurrence.md) | [Back to README](../README.md) | [Next: Solving Recurrences â†’](05-solving-recurrences.md)
