# Chapter 6.4: Advanced Techniques for Trigonometric Equations

## Overview

This chapter covers advanced methods for solving trigonometric equations that don't fit the simple patterns from previous chapters. We'll explore equations requiring factorization, transformation to a single function, homogeneous equations, and the auxiliary angle method.

---

## ğŸ“ Method 1: Factorization

### When to Use

When the equation can be factored into simpler trigonometric expressions.

### Example 1: sin x cos x = 0

**Solution:**
$$\sin x \cos x = 0$$
$$\sin x = 0 \quad \text{or} \quad \cos x = 0$$

sin x = 0: x = nÏ€
cos x = 0: x = (2n + 1)Ï€/2

**Combined solution:** x = nÏ€/2, n âˆˆ â„¤

### Example 2: sin 2x = sin x

**Solution:**
$$\sin 2x - \sin x = 0$$
$$2\sin x \cos x - \sin x = 0$$
$$\sin x(2\cos x - 1) = 0$$

sin x = 0: x = nÏ€
cos x = 1/2: x = 2nÏ€ Â± Ï€/3

### Example 3: cos 2x = cos x

**Solution:**
$$\cos 2x - \cos x = 0$$
$$2\cos^2 x - 1 - \cos x = 0$$
$$2\cos^2 x - \cos x - 1 = 0$$
$$(2\cos x + 1)(\cos x - 1) = 0$$

cos x = -1/2: x = 2nÏ€ Â± 2Ï€/3
cos x = 1: x = 2nÏ€

---

## ğŸ“ Method 2: Equations of the Form a sin x + b cos x = c

### The Auxiliary Angle Method

For equations of the form **a sin x + b cos x = c**, we use:

$$a\sin x + b\cos x = R\sin(x + \phi)$$

where:
$$R = \sqrt{a^2 + b^2}$$
$$\tan\phi = \frac{b}{a}$$

```
    â”Œâ”€â”€â”€â”€â”€â”€â”€â”€â”€â”€â”€â”€â”€â”€â”€â”€â”€â”€â”€â”€â”€â”€â”€â”€â”€â”€â”€â”€â”€â”€â”€â”€â”€â”€â”€â”€â”€â”€â”€â”€â”€â”€â”€â”€â”€â”€â”€â”€â”€â”€â”€â”€â”€â”€â”€â”€â”€â”€â”€â”€â”€â”€â”€â”€â”
    â”‚           AUXILIARY ANGLE METHOD                               â”‚
    â”œâ”€â”€â”€â”€â”€â”€â”€â”€â”€â”€â”€â”€â”€â”€â”€â”€â”€â”€â”€â”€â”€â”€â”€â”€â”€â”€â”€â”€â”€â”€â”€â”€â”€â”€â”€â”€â”€â”€â”€â”€â”€â”€â”€â”€â”€â”€â”€â”€â”€â”€â”€â”€â”€â”€â”€â”€â”€â”€â”€â”€â”€â”€â”€â”€â”¤
    â”‚                                                                â”‚
    â”‚  a sin x + b cos x = c                                        â”‚
    â”‚                                                                â”‚
    â”‚  Step 1: Calculate R = âˆš(aÂ² + bÂ²)                             â”‚
    â”‚                                                                â”‚
    â”‚  Step 2: Find Ï† where tan Ï† = b/a                             â”‚
    â”‚                                                                â”‚
    â”‚  Step 3: Rewrite as R sin(x + Ï†) = c                          â”‚
    â”‚                                                                â”‚
    â”‚  Step 4: sin(x + Ï†) = c/R                                     â”‚
    â”‚                                                                â”‚
    â”‚  Step 5: Check if |c/R| â‰¤ 1 (solution exists)                 â”‚
    â”‚                                                                â”‚
    â”‚  Step 6: Solve x + Ï† = general solution                       â”‚
    â”‚                                                                â”‚
    â””â”€â”€â”€â”€â”€â”€â”€â”€â”€â”€â”€â”€â”€â”€â”€â”€â”€â”€â”€â”€â”€â”€â”€â”€â”€â”€â”€â”€â”€â”€â”€â”€â”€â”€â”€â”€â”€â”€â”€â”€â”€â”€â”€â”€â”€â”€â”€â”€â”€â”€â”€â”€â”€â”€â”€â”€â”€â”€â”€â”€â”€â”€â”€â”€â”˜
```

### Alternative Form

$$a\sin x + b\cos x = R\cos(x - \psi)$$

where tan Ïˆ = a/b

### Example 4: sin x + cos x = 1

**Solution:**
Here a = 1, b = 1.

$$R = \sqrt{1^2 + 1^2} = \sqrt{2}$$
$$\tan\phi = \frac{1}{1} = 1 \Rightarrow \phi = \frac{\pi}{4}$$

Rewrite:
$$\sqrt{2}\sin\left(x + \frac{\pi}{4}\right) = 1$$
$$\sin\left(x + \frac{\pi}{4}\right) = \frac{1}{\sqrt{2}}$$

Let Î¸ = x + Ï€/4:
$$\sin\theta = \frac{1}{\sqrt{2}}$$
$$\theta = n\pi + (-1)^n \cdot \frac{\pi}{4}$$

Therefore:
$$x + \frac{\pi}{4} = n\pi + (-1)^n \cdot \frac{\pi}{4}$$
$$x = n\pi + (-1)^n \cdot \frac{\pi}{4} - \frac{\pi}{4}$$

**Simplifying:**
- For n even: x = 2kÏ€ + Ï€/4 - Ï€/4 = 2kÏ€ â†’ x = 0, 2Ï€, 4Ï€, ...
- For n odd: x = (2k+1)Ï€ - Ï€/4 - Ï€/4 = (2k+1)Ï€ - Ï€/2 â†’ x = Ï€/2, 5Ï€/2, ...

**Solutions in [0, 2Ï€]: x = 0, Ï€/2**

### Example 5: âˆš3 sin x + cos x = 2

**Solution:**
Here a = âˆš3, b = 1.

$$R = \sqrt{3 + 1} = 2$$
$$\tan\phi = \frac{1}{\sqrt{3}} \Rightarrow \phi = \frac{\pi}{6}$$

Rewrite:
$$2\sin\left(x + \frac{\pi}{6}\right) = 2$$
$$\sin\left(x + \frac{\pi}{6}\right) = 1$$
$$x + \frac{\pi}{6} = 2n\pi + \frac{\pi}{2}$$
$$x = 2n\pi + \frac{\pi}{2} - \frac{\pi}{6}$$
$$x = 2n\pi + \frac{\pi}{3}$$

### Example 6: sin x + âˆš3 cos x = 1

**Solution:**
Here a = 1, b = âˆš3.

$$R = \sqrt{1 + 3} = 2$$
$$\tan\phi = \sqrt{3} \Rightarrow \phi = \frac{\pi}{3}$$

$$2\sin\left(x + \frac{\pi}{3}\right) = 1$$
$$\sin\left(x + \frac{\pi}{3}\right) = \frac{1}{2}$$
$$x + \frac{\pi}{3} = n\pi + (-1)^n \cdot \frac{\pi}{6}$$
$$x = n\pi + (-1)^n \cdot \frac{\pi}{6} - \frac{\pi}{3}$$

---

## ğŸ“ Method 3: Homogeneous Equations

### Definition

A **homogeneous equation** in sin x and cos x has all terms of the same degree.

### Example: Linear Homogeneous (Degree 1)

a sin x + b cos x = 0

**Solution:** Divide by cos x:
$$a\tan x + b = 0$$
$$\tan x = -\frac{b}{a}$$

### Example 7: 3 sin x - 4 cos x = 0

**Solution:**
Divide by cos x (assuming cos x â‰  0):
$$3\tan x - 4 = 0$$
$$\tan x = \frac{4}{3}$$
$$x = n\pi + \arctan\left(\frac{4}{3}\right)$$

We need to check if cos x = 0 gives solutions:
If cos x = 0, then sin x = Â±1, and 3(Â±1) - 4(0) = Â±3 â‰  0.
So cos x = 0 is not a solution.

### Example: Quadratic Homogeneous (Degree 2)

a sinÂ²x + b sin x cos x + c cosÂ²x = 0

**Solution:** Divide by cosÂ²x:
$$a\tan^2 x + b\tan x + c = 0$$

### Example 8: 2sinÂ²x - 5sin x cos x + 2cosÂ²x = 0

**Solution:**
Divide by cosÂ²x:
$$2\tan^2 x - 5\tan x + 2 = 0$$
$$(2\tan x - 1)(\tan x - 2) = 0$$
$$\tan x = \frac{1}{2} \quad \text{or} \quad \tan x = 2$$

$$x = n\pi + \arctan\left(\frac{1}{2}\right) \quad \text{or} \quad x = n\pi + \arctan(2)$$

---

## ğŸ“ Method 4: Using Sum-to-Product Formulas

### Example 9: sin 3x + sin x = 0

**Solution:**
Using sum-to-product:
$$2\sin\left(\frac{3x + x}{2}\right)\cos\left(\frac{3x - x}{2}\right) = 0$$
$$2\sin 2x \cos x = 0$$

sin 2x = 0: 2x = nÏ€ â†’ x = nÏ€/2
cos x = 0: x = (2n + 1)Ï€/2

**Combined:** x = nÏ€/2

### Example 10: cos 5x - cos x = 0

**Solution:**
Using sum-to-product:
$$-2\sin\left(\frac{5x + x}{2}\right)\sin\left(\frac{5x - x}{2}\right) = 0$$
$$-2\sin 3x \sin 2x = 0$$

sin 3x = 0: 3x = nÏ€ â†’ x = nÏ€/3
sin 2x = 0: 2x = nÏ€ â†’ x = nÏ€/2

**Combined solution:** Need to find the union of both sets.

---

## ğŸ“ Method 5: Substitution t = tan(x/2)

### Weierstrass Substitution

Let t = tan(x/2). Then:

$$\sin x = \frac{2t}{1 + t^2}$$
$$\cos x = \frac{1 - t^2}{1 + t^2}$$

This converts all trigonometric equations to polynomial equations in t.

### Example 11: 5cos x + 12sin x = 13

**Solution using auxiliary angle:**
R = âˆš(25 + 144) = 13
$$13\sin(x + \phi) = 13$$
$$\sin(x + \phi) = 1$$

where tan Ï† = 5/12.

$$x + \phi = 2n\pi + \frac{\pi}{2}$$
$$x = 2n\pi + \frac{\pi}{2} - \arctan\left(\frac{5}{12}\right)$$

---

## ğŸ“ Method 6: Equations with Multiple Angles

### Example 12: sin 2x = cos x

**Solution:**
$$2\sin x \cos x = \cos x$$
$$\cos x(2\sin x - 1) = 0$$

cos x = 0: x = (2n + 1)Ï€/2
sin x = 1/2: x = nÏ€ + (-1)â¿(Ï€/6)

### Example 13: cos 3x = 4cosÂ³x - 3cos x (Verification)

This is the triple angle identity, so:
$$4\cos^3 x - 3\cos x = 4\cos^3 x - 3\cos x$$

This is true for all x (identity, not equation).

---

## ğŸ“Š Summary of Methods

```
    â”Œâ”€â”€â”€â”€â”€â”€â”€â”€â”€â”€â”€â”€â”€â”€â”€â”€â”€â”€â”€â”€â”€â”€â”€â”€â”€â”€â”€â”€â”€â”€â”€â”€â”€â”€â”€â”€â”€â”€â”€â”€â”€â”€â”€â”€â”€â”€â”€â”€â”€â”€â”€â”€â”€â”€â”€â”€â”€â”€â”€â”€â”€â”€â”€â”€â”
    â”‚                    CHOOSING THE RIGHT METHOD                   â”‚
    â”œâ”€â”€â”€â”€â”€â”€â”€â”€â”€â”€â”€â”€â”€â”€â”€â”€â”€â”€â”€â”€â”€â”€â”€â”€â”€â”€â”€â”€â”€â”€â”€â”€â”€â”€â”€â”€â”€â”€â”€â”€â”€â”€â”€â”€â”€â”€â”€â”€â”€â”€â”€â”€â”€â”€â”€â”€â”€â”€â”€â”€â”€â”€â”€â”€â”¤
    â”‚                                                                â”‚
    â”‚  Equation Type                        Method                   â”‚
    â”‚  â”€â”€â”€â”€â”€â”€â”€â”€â”€â”€â”€â”€â”€                        â”€â”€â”€â”€â”€â”€                   â”‚
    â”‚                                                                â”‚
    â”‚  Can be factored                      Factor, set each = 0    â”‚
    â”‚                                                                â”‚
    â”‚  a sin x + b cos x = c               Auxiliary angle          â”‚
    â”‚                                                                â”‚
    â”‚  All terms same degree                Divide by cosâ¿x         â”‚
    â”‚  (homogeneous)                                                â”‚
    â”‚                                                                â”‚
    â”‚  sin A + sin B or cos A + cos B       Sum-to-product          â”‚
    â”‚                                                                â”‚
    â”‚  Multiple angles like sin 2x          Use double angle        â”‚
    â”‚                                       formulas                â”‚
    â”‚                                                                â”‚
    â”‚  Complex rational expressions         t = tan(x/2)            â”‚
    â”‚                                                                â”‚
    â””â”€â”€â”€â”€â”€â”€â”€â”€â”€â”€â”€â”€â”€â”€â”€â”€â”€â”€â”€â”€â”€â”€â”€â”€â”€â”€â”€â”€â”€â”€â”€â”€â”€â”€â”€â”€â”€â”€â”€â”€â”€â”€â”€â”€â”€â”€â”€â”€â”€â”€â”€â”€â”€â”€â”€â”€â”€â”€â”€â”€â”€â”€â”€â”€â”˜
```

---

## ğŸ“‹ Summary Table

### Method Quick Reference

| Method | When to Use | Key Step |
|--------|-------------|----------|
| Factorization | Terms share common factor | Factor, solve each |
| Auxiliary Angle | a sin x + b cos x = c | R = âˆš(aÂ²+bÂ²), tan Ï† = b/a |
| Homogeneous | All terms same degree | Divide by cosâ¿x |
| Sum-to-Product | Sum/diff of same function | Apply Sâ†’P formula |
| Multiple Angle | Contains sin 2x, cos 2x, etc. | Use double/triple formulas |
| Weierstrass | Complex expressions | t = tan(x/2) |

### Auxiliary Angle Formulas

| Form | Transformation |
|------|----------------|
| a sin x + b cos x | R sin(x + Ï†) where R = âˆš(aÂ²+bÂ²), tan Ï† = b/a |
| a sin x + b cos x | R cos(x - Ïˆ) where R = âˆš(aÂ²+bÂ²), tan Ïˆ = a/b |
| a cos x + b sin x | R cos(x - Ï†) where R = âˆš(aÂ²+bÂ²), tan Ï† = b/a |

---

## â“ Quick Revision Questions

1. **Solve: sin x cos x = 0 in [0, 2Ï€].**

2. **Solve: sin x + cos x = âˆš2.**

3. **Solve: sin x - âˆš3 cos x = 1 (general solution).**

4. **Solve: 3sinÂ²x + 4sin x cos x - cosÂ²x = 0 in [0, Ï€].**

5. **Solve: sin 5x + sin 3x = 0 (general solution).**

6. **For the equation a sin x + b cos x = c, what is the condition for a solution to exist?**

<details>
<summary>Click to see answers</summary>

1. sin x cos x = 0  
   sin x = 0 or cos x = 0  
   In [0, 2Ï€]:  
   sin x = 0: x = 0, Ï€, 2Ï€  
   cos x = 0: x = Ï€/2, 3Ï€/2  
   **Solutions: x = 0, Ï€/2, Ï€, 3Ï€/2, 2Ï€**

2. sin x + cos x = âˆš2  
   R = âˆš2, tan Ï† = 1, Ï† = Ï€/4  
   âˆš2 sin(x + Ï€/4) = âˆš2  
   sin(x + Ï€/4) = 1  
   x + Ï€/4 = 2nÏ€ + Ï€/2  
   **x = 2nÏ€ + Ï€/4**

3. sin x - âˆš3 cos x = 1  
   a = 1, b = -âˆš3, R = 2  
   tan Ï† = -âˆš3/1 = -âˆš3, so Ï† = -Ï€/3  
   2 sin(x - Ï€/3) = 1  
   sin(x - Ï€/3) = 1/2  
   x - Ï€/3 = nÏ€ + (-1)â¿(Ï€/6)  
   **x = nÏ€ + (-1)â¿(Ï€/6) + Ï€/3**

4. 3sinÂ²x + 4sin x cos x - cosÂ²x = 0  
   Divide by cosÂ²x:  
   3tanÂ²x + 4tan x - 1 = 0  
   tan x = (-4 Â± âˆš(16 + 12))/6 = (-4 Â± âˆš28)/6 = (-4 Â± 2âˆš7)/6 = (-2 Â± âˆš7)/3  
   
   tan x = (-2 + âˆš7)/3 â‰ˆ 0.215 â†’ x â‰ˆ 0.212 rad  
   tan x = (-2 - âˆš7)/3 â‰ˆ -1.549 â†’ x â‰ˆ 2.142 rad (Ï€ - 1.00)  
   
   **In [0, Ï€]: x = arctan((-2+âˆš7)/3) and x = Ï€ + arctan((-2-âˆš7)/3)**

5. sin 5x + sin 3x = 0  
   2 sin 4x cos x = 0  
   sin 4x = 0 or cos x = 0  
   
   4x = nÏ€ â†’ x = nÏ€/4  
   x = (2n+1)Ï€/2  
   
   **General solution: x = nÏ€/4** (the cos x = 0 solutions are included as n = 2, 6, 10, ...)

6. For a sin x + b cos x = c to have solutions:  
   We rewrite as R sin(x + Ï†) = c where R = âˆš(aÂ² + bÂ²)  
   Then sin(x + Ï†) = c/R  
   For sin to have solutions, we need |c/R| â‰¤ 1  
   So |c| â‰¤ R  
   **Condition: |c| â‰¤ âˆš(aÂ² + bÂ²)**  
   Or equivalently: cÂ² â‰¤ aÂ² + bÂ²

</details>

---

## Navigation

| Previous | Up | Next |
|----------|-------|------|
| [â† 6.3 Quadratic Equations](03-quadratic-equations.md) | [Unit 6 Index](README.md) | [Unit 7: Inverse Functions â†’](../07-Inverse-Trigonometric-Functions/README.md) |

---

[â† Back to Main Index](../README.md)
